@prefix : <http://ccd-tna.kartography.cloud/resource/> .
@prefix rs: <http://www.researchspace.org/ontology/> .
@prefix User: <http://www.researchspace.org/resource/user/> .
@prefix Help: <http://help.researchspace.org/resource/> .
@prefix Platform: <http://www.researchspace.org/resource/system/> .
@prefix owl: <http://www.w3.org/2002/07/owl#> .
@prefix xsd: <http://www.w3.org/2001/XMLSchema#> .
@prefix skos: <http://www.w3.org/2004/02/skos/core#> .
@prefix rdfs: <http://www.w3.org/2000/01/rdf-schema#> .
@prefix crmdig: <http://www.ics.forth.gr/isl/CRMdig/> .
@prefix rsp: <http://www.researchspace.org/resource/> .
@prefix rshelp: <http://researchspace.org/help/> .
@prefix crmsci: <http://www.ics.forth.gr/isl/CRMsci/> .
@prefix crmgeo: <http://www.ics.forth.gr/isl/CRMgeo/> .
@prefix sp: <http://spinrdf.org/sp#> .
@prefix prov: <http://www.w3.org/ns/prov#> .
@prefix crminfluence: <http://www.cidoc-crm.org/cidoc-crm/influence/> .
@prefix crm: <http://www.cidoc-crm.org/cidoc-crm/> .
@prefix crminf: <http://www.ics.forth.gr/isl/CRMinf/> .
@prefix Admin: <http://www.researchspace.org/resource/admin/> .
@prefix bds: <http://www.bigdata.com/rdf/search#> .
@prefix rdf: <http://www.w3.org/1999/02/22-rdf-syntax-ns#> .
@prefix crmba: <http://www.cidoc-crm.org/cidoc-crm/CRMba/> .
@prefix ontodia: <http://ontodia.org/schema/v1#> .
@prefix crmarchaeo: <http://www.cidoc-crm.org/cidoc-crm/CRMarchaeo/> .
@prefix forms: <http://www.researchspace.org/resource/system/forms/> .
@prefix frbroo: <http://iflastandards.info/ns/fr/frbr/frbroo/> .

crmdig:context {
  crmdig:L1_digitized a owl:ObjectProperty;
    rdfs:domain crmdig:D2_Digitization_Process;
    rdfs:subPropertyOf crm:P39_measured;
    rdfs:range crm:E18_Physical_Thing;
    rdfs:comment """This property associates an instance of D2 Digitization Process with an instance of E18 Physical Thing which is a material thing.  
This property is a specialisation of P39 measured (was measured by).
"""@en .
  
  crmdig:D29_Annotation_Object a owl:Class;
    rdfs:subClassOf crm:E89_Propositional_Object;
    rdfs:comment """This class comprises objects that make propositions about other artefacts. 
	Instances of this class are not the attributes themselves, by which things are annotated, 
	but represent the connection between the concepts related in a proposition, and the activities of creation, modification and deletion. 
	"""@en .
  
  crmdig:D7_Digital_Machine_Event a owl:Class;
    rdfs:comment """This class comprises events that happen on physical digital devices following a human activity that intentionally caused its 
	immediate or delayed initiation and results in the creation of a new instance of D1 Digital Object on behalf of the human actor. 
	The input of a D7 Digital Machine Event may be parameter settings and/or data to be processed. 
	Some D7 Digital Machine Events may form part of a wider E65 Creation event. 
	In this case, all machine output of the partial events is regarded as creation of the overall activity.
	"""@en;
    rdfs:subClassOf crm:E11_Modification, crm:E65_Creation .
  
  crmdig:L10i_was_input_of a owl:ObjectProperty;
    rdfs:domain crmdig:D1_Digital_Object;
    rdfs:subPropertyOf crm:P16i_was_used_for;
    rdfs:range crmdig:D7_Digital_Machine_Event .
  
  crmdig:D23_Room a owl:Class;
    rdfs:subClassOf crm:E53_Place;
    rdfs:comment ""@en .
  
  crmdig:D1_Digital_Object a owl:Class;
    rdfs:subClassOf crm:E73_Information_Object;
    rdfs:comment """This class comprises identifiable immaterial items that can be represented as sets of bit sequences, 
	such as data sets, e-texts, images, audio or video items, software, etc., and are documented as single units. 
	Any aggregation of instances of D1 Digital Object into a whole treated as single unit is also regarded as an instance of D1 Digital Object. 
	This means that for instance, the content of a DVD, an XML file on it, and an element of this file, are regarded as distinct instances of 
	D1 Digital Object, mutually related by the P106 is composed of (forms part of) property.
A D1 Digital Object does not depend on a specific physical carrier, and it can exist on one or more carriers simultaneously.
"""@en .
  
  crmdig:D30_Annotation_Event a owl:Class;
    rdfs:subClassOf crm:E65_Creation;
    rdfs:comment """This class comprises events that describe the creation of associations (Annotation Objects) between objects 
	or areas of objects of the Repository, with other objects or regions or persons, places, events. It is the event that creates the Annotation Object."""@en .
  
  crmdig:L11_had_output a owl:ObjectProperty;
    rdfs:domain crmdig:D7_Digital_Machine_Event;
    rdfs:subPropertyOf crm:P94_has_created;
    rdfs:comment """This property associates an instance of D7 Digital Machine Event with an instance of D1 Digital Object
 which is the output of the activity.  
This property is a specialisation of P94 has created (was created by)."""@en;
    rdfs:range crmdig:D1_Digital_Object .
  
  <http://www.ics.forth.gr/isl/CRMdig/> a owl:Ontology, prov:Entity, <http://www.w3.org/ns/ldp#Resource>;
    owl:versionInfo "3.2.1"@en;
    rdfs:comment "An Extension of CIDOC-CRM to support provenance metadata"@en;
    prov:wasAttributedTo User:admin;
    prov:generatedAtTime "2021-10-04T05:27:55.354Z"^^xsd:dateTime;
    rdfs:label "CRMdig v3.2.1"@en .
  
  crmdig:D9_Data_Object a owl:Class;
    rdfs:subClassOf crmdig:D1_Digital_Object, crm:E54_Dimension;
    rdfs:comment """This class comprises instances of D1 Digital Object that are the direct result of a digital 
	measurement or a formal derivative of it, containing quantitative properties of some physical things or other constellations of matter.
	"""@en .
  
  crmdig:L13i_parameters_for a owl:ObjectProperty;
    rdfs:domain crmdig:D1_Digital_Object;
    rdfs:range crmdig:D10_Software_Execution;
    rdfs:subPropertyOf crmdig:L10i_was_input_of .
  
  crmdig:D10_Software_Execution a owl:Class;
    rdfs:comment """This class comprises events by which a digital device runs a software program or a series of  computing 
	operations on a digital object  as a single task, which is completely determined by its digital input, 
	the software and the generic properties of the device. 
	"""@en;
    rdfs:subClassOf crmdig:D7_Digital_Machine_Event .
  
  crmdig:L12i_was_device_for a owl:ObjectProperty;
    rdfs:domain crmdig:D8_Digital_Device;
    rdfs:range crmdig:D7_Digital_Machine_Event;
    rdfs:subPropertyOf crm:P12i_was_present_at .
  
  crmdig:L11i_was_output_of a owl:ObjectProperty;
    rdfs:subPropertyOf crm:P94i_was_created_by;
    rdfs:domain crmdig:D1_Digital_Object;
    rdfs:range crmdig:D7_Digital_Machine_Event .
  
  crmdig:D14_Software a owl:Class;
    rdfs:comment """This class comprises software codes,computer programs,procedures, and functions that are
	used to operate a system of digital objects. """@en;
    rdfs:subClassOf crmdig:D1_Digital_Object .
  
  crmdig:D35_Area a owl:Class;
    rdfs:subClassOf crmdig:D1_Digital_Object, crm:E26_Physical_Feature;
    rdfs:comment """This class describes a part (of any shape or size) of interest in basically any media object stored in the Object Repository,
	i.e., a text, an image, a video or a 3D model. It points to content consisting of just a portion or area of a file. 
In some contexts, however, the area can also point to content represented by an integral (i.e., proper) file. It is equal to the METS AREA element """@en .
  
  crmdig:D2_Digitization_Process a owl:Class;
    rdfs:subClassOf crmdig:D11_Digital_Measurement_Event;
    rdfs:comment """This class comprises events that result in the creation of instances of D9 Data Object that 
	represent the appearance and/or form of an instance of E18 Physical Thing such as paper documents, statues, buildings, paintings, etc. 
	A particular case is the analogue-to-digital conversion of audiovisual material.
	This class represents the transition from a material thing to an immaterial representation of it. 
	The characteristic subsequent processing steps on digital objects are regarded as instances of D3 Formal Derivation.
"""@en .
  
  crmdig:D8_Digital_Device a owl:Class;
    rdfs:subClassOf crm:E22_Man-Made_Object;
    rdfs:comment """This class comprises identifiable material items such as computers, scanners, cameras, etc. that 
	have the capability to process or produce instances of  D1 Digital Object.
	"""@en .
  
  crmdig:L12_happened_on_device a owl:ObjectProperty;
    rdfs:subPropertyOf crm:P12_occurred_in_the_presence_of;
    rdfs:range crmdig:D8_Digital_Device;
    rdfs:domain crmdig:D7_Digital_Machine_Event;
    rdfs:comment """This property associates an instance of D7 Digital Machine Event  with an object,
 the D8 Digital Device, which happened with, e.g  a capturing event that happened on/with a digital camera, etc. 
This property is a specialisation of P12 occurred in the presence of (was present at)."""@en .
  
  crmdig:D11_Digital_Measurement_Event a owl:Class;
    rdfs:subClassOf crmdig:D7_Digital_Machine_Event, crm:E16_Measurement;
    rdfs:comment """This class comprises actions measuring physical properties using a digital device, 
	that are determined by a systematic procedure and creates an instance of D9 Data Object, 
	which is stored on an instance of D13 Digital Information Carrier. 
	In contrast to instances of D10 Software Execution, environmental factors have an intended influence on the outcome of an instance of D11 Digital Measurement Event. 
	Measurement devices may include running distinct software, such as the RAW to JPEG conversion in digital cameras. 
	In this case, the event is regarded as instance of both classes, D10 Software Execution and D11 Digital Measurement Event.
	"""@en .
  
  crmdig:D21_Person_Name a owl:Class;
    rdfs:comment """This class comprises the proper noun name that identifies a person that acts
as an entity."""@en;
    rdfs:subClassOf crm:E82_Actor_Appellation .
  
  crmdig:D12_Data_Transfer_Event a owl:Class;
    rdfs:comment """This class comprises events that transfer a digital object from one digital carrier to another. 
	Normally, the digital object remains the same. If in general or by observation the transfer implies or has 
	implied some data corruption, the change of the digital objects may be documented distinguishing input and output 
	rather than instantiating the property L14 transferred (was transferred by). 
	"""@en;
    rdfs:subClassOf crmdig:D7_Digital_Machine_Event .
  
  crmdig:D13_Digital_Information_Carrier a owl:Class;
    rdfs:subClassOf crm:E84_Information_Carrier;
    rdfs:comment """This class comprises all instances of E84 Information Carrier that are explicitly designed to be 
	used as persistent digital physical carriers of instances of D1 Digital Object. 
	A D13 Digital Information Carrier may or may not contain information, e.g., an empty diskette.
	"""@en .
  
  crmdig:L13_used_parameters a owl:ObjectProperty;
    rdfs:comment """This property associates an instance of D10 Software Execution with a digital object
 used as a parameter during the process.This property is a specialisation of L1O had input (was input of)."""@en;
    rdfs:range crmdig:D1_Digital_Object;
    rdfs:subPropertyOf crmdig:L10_had_input;
    rdfs:domain crmdig:D10_Software_Execution .
  
  crmdig:L10_had_input a owl:ObjectProperty;
    rdfs:comment """This property associates an instance of D7 Digital Machine Event with an instance of D1 Digital Object
 which is the input used to specify the machine action.  
This property is a specialisation of P16 used specific object(was used for).
"""@en;
    rdfs:range crmdig:D1_Digital_Object;
    rdfs:domain crmdig:D7_Digital_Machine_Event;
    rdfs:subPropertyOf crm:P16_used_specific_object .
  
  crmdig:D3_Formal_Derivation a owl:Class;
    rdfs:comment """This class comprises events that result in the creation of a D1 Digital Object from another one following a deterministic algorithm, 
	such that the resulting instance of digital object shares representative properties with the original object. 
	In other words, this class describes the transition from an immaterial object referred to by property L21 used as derivation source (was derivation source for) 
	to another immaterial object referred to by property L22 created derivative (was derivative created by) preserving the 
	representation of some things but in a different form. Characteristic examples are colour corrections, contrast changes and resizing of images.
	"""@en;
    rdfs:subClassOf crmdig:D10_Software_Execution .
  
  <http://researchspace.org/container/rootContainer/ontologyContainer> <http://www.w3.org/ns/ldp#contains>
      <http://www.ics.forth.gr/isl/CRMdig/> .
  
  crmdig:L23i_was_software_or_firmware_used_by a owl:ObjectProperty;
    rdfs:subPropertyOf crm:P16i_was_used_for;
    rdfs:range crmdig:D7_Digital_Machine_Event;
    rdfs:domain crmdig:D14_Software .
  
  crmdig:L29i_is_responsible_organization_for a owl:ObjectProperty;
    rdfs:domain crm:E40_Legal_Body;
    rdfs:subPropertyOf crm:P14i_performed;
    rdfs:range crm:E7_Activity .
  
  crmdig:L30i_is_operator_of a owl:ObjectProperty;
    rdfs:range crm:E7_Activity;
    rdfs:domain crm:E21_Person;
    rdfs:subPropertyOf crm:P14i_performed .
  
  crmdig:L4_has_preferred_label a owl:DatatypeProperty;
    rdfs:range xsd:string;
    rdfs:subPropertyOf rdfs:label;
    rdfs:comment """This property associates an instance of E1 Entity with an instance of resource used as a preferred lexical label.  
This property is a specialisation of rdf schema label.
"""@en;
    rdfs:domain crm:E1_CRM_Entity .
  
  crmdig:L43_annotates a owl:ObjectProperty;
    rdfs:range crm:E1_CRM_Entity;
    rdfs:comment """This property describes the associations between objects or areas of objects of the RI, 
with other objects or regions or persons, places, events.."""@en;
    rdfs:domain crmdig:D29_Annotation_Object .
  
  crmdig:L24_created_logfile a owl:ObjectProperty;
    rdfs:comment "This property identifies the logfile that was created by a D10 Software Execution in order to record all the activities in the system."@en;
    rdfs:range crmdig:D1_Digital_Object;
    rdfs:domain crmdig:D10_Software_Execution;
    rdfs:subPropertyOf crmdig:L11_had_output .
  
  crmdig:L24i_was_logfile_created_by a owl:ObjectProperty;
    rdfs:range crmdig:D10_Software_Execution;
    rdfs:domain crmdig:D1_Digital_Object;
    rdfs:subPropertyOf crmdig:L11i_was_output_of .
  
  crmdig:L31_has_starting_date-time a owl:ObjectProperty;
    rdfs:range xsd:dateTime;
    rdfs:domain crm:E5_Event;
    rdfs:subPropertyOf crm:P82a_begin_of_the_begin;
    rdfs:comment """This property allows the starting point for a D7 Digital Machine Event to be situated.   
This property expresses the approximation of the starting date of a time span."""@en .
  
  crmdig:L35_has_commissioner a owl:ObjectProperty;
    rdfs:comment """This property describes the participation of a Legal Body in being commissioner for the outcome of a specific activity.
This property is a specialisation of L29_has_responsible_organization."""@en;
    rdfs:subPropertyOf crmdig:L29_has_responsible_organization;
    rdfs:range crm:E40_Legal_Body;
    rdfs:domain crm:E7_Activity .
  
  crmdig:L2i_was_source_for a owl:ObjectProperty;
    rdfs:range crmdig:D10_Software_Execution;
    rdfs:domain crmdig:D1_Digital_Object;
    rdfs:subPropertyOf crmdig:L10i_was_input_of .
  
  crmdig:L48_created_annotation a owl:ObjectProperty;
    rdfs:subPropertyOf crm:P94_has_created;
    rdfs:domain crmdig:D30_Annotation_Event;
    rdfs:range crmdig:D29_Annotation_Object;
    rdfs:comment """This property identifies the D29 Annotation Object (associations) that came into existence as a result of a D30 Annotation Event.
This property is a specialisation of P94 has created."""@en .
  
  crmdig:L47_has_comment a owl:DatatypeProperty;
    rdfs:range xsd:string;
    rdfs:subPropertyOf crm:P3_has_note;
    rdfs:comment "This property is a specialisation of P3 has note and associates a comment with an instance of an object E1 CRM Entity."@en;
    rdfs:domain crm:E1_CRM_Entity .
  
  crmdig:L34i_is_contractor_for a owl:ObjectProperty;
    rdfs:subPropertyOf crmdig:L29i_is_responsible_organization_for;
    rdfs:range crm:E7_Activity;
    rdfs:domain crm:E40_Legal_Body .
  
  crmdig:L34_has_contractor a owl:ObjectProperty;
    rdfs:domain crm:E7_Activity;
    rdfs:comment """This property describes the participation of a Legal Body in being contractor for the outcome of a specific activity.
This property is a specialisation of L29_has_responsible_organization."""@en;
    rdfs:subPropertyOf crmdig:L29_has_responsible_organization;
    rdfs:range crm:E40_Legal_Body .
  
  crmdig:L35i_is_commissioner_for a owl:ObjectProperty;
    rdfs:domain crm:E40_Legal_Body;
    rdfs:subPropertyOf crmdig:L29i_is_responsible_organization_for;
    rdfs:range crm:E7_Activity .
  
  crmdig:L33i_is_maker_of a owl:ObjectProperty;
    rdfs:domain crm:E39_Actor;
    rdfs:range crm:E72_Legal_Object .
  
  crmdig:L29_has_responsible_organization a owl:ObjectProperty;
    rdfs:comment """This property describes the participation of a Legal Body in being responsible for the outcome of a specific activity.
This property is a specialisation of P14 carried out by."""@en;
    rdfs:range crm:E40_Legal_Body;
    rdfs:subPropertyOf crm:P14_carried_out_by;
    rdfs:domain crm:E7_Activity .
  
  crmdig:L49_is_primary_area_of a owl:ObjectProperty;
    rdfs:comment """This property describes the association between a particular area declared in an original digital object.
This property is a specialisation of P106 is composed of."""@en;
    rdfs:domain crmdig:D35_Area;
    rdfs:subPropertyOf crm:P106i_forms_part_of;
    rdfs:range crmdig:D1_Digital_Object .
  
  crmdig:L48i_was_annotation_created_by a owl:ObjectProperty;
    rdfs:subPropertyOf crm:P94i_was_created_by;
    rdfs:range crmdig:D30_Annotation_Event;
    rdfs:domain crmdig:D29_Annotation_Object .
  
  crmdig:L30_has_operator a owl:ObjectProperty;
    rdfs:comment """This property describes the activity that is being operated by a person.
This property is a specialisation of P14 carried out by."""@en;
    rdfs:range crm:E21_Person;
    rdfs:subPropertyOf crm:P14_carried_out_by;
    rdfs:domain crm:E7_Activity .
  
  crmdig:L32_has_ending_date-time a owl:ObjectProperty;
    rdfs:range xsd:dateTime;
    rdfs:domain crm:E5_Event;
    rdfs:subPropertyOf crm:P82b_end_of_the_end;
    rdfs:comment """This property allows the ending point for a D7 Digital Machine Event to be situated.   
This property expresses the approximation of the ending date of a time span."""@en .
  
  crmdig:L23_used_software_or_firmware a owl:ObjectProperty;
    rdfs:subPropertyOf crm:P16_used_specific_object;
    rdfs:comment """This property associates an instance of D7 Digital Machine Event with the instance of D14 Software that had used.
This property is a specialisation of P16 used specific object."""@en;
    rdfs:range crmdig:D14_Software;
    rdfs:domain crmdig:D7_Digital_Machine_Event .
  
  crmdig:L33_has_maker a owl:ObjectProperty;
    rdfs:domain crm:E72_Legal_Object;
    rdfs:comment """This property identifies the maker, the actor who is responsible for the production of a device,
 a computer, a digital camera, any kind of a machine that has been produced.
This property is a shortcut of a more fully developed path from CRM E12 Production:P108 has produced:E24 Physical Man-Made Thing. 
In this case, there is no need to describe the more detailed property through a production event,so L33 has maker is reccomended to be used instead. """@en;
    rdfs:range crm:E39_Actor .
  
  crmdig:L43i_is_annotated_by a owl:ObjectProperty;
    rdfs:domain crm:E1_CRM_Entity;
    rdfs:range crmdig:D29_Annotation_Object .
  
  crmdig:L50i_has_propagated_area a owl:ObjectProperty;
    rdfs:subPropertyOf crm:P106_is_composed_of;
    rdfs:domain crmdig:D1_Digital_Object;
    rdfs:range crmdig:D35_Area .
  
  crmdig:L51_has_first_name a owl:DatatypeProperty;
    rdfs:subPropertyOf rdfs:label;
    rdfs:range xsd:string;
    rdfs:domain crmdig:D21_Person_Name;
    rdfs:comment "This property defines a personal name used to identify a person."@en .
  
  crmdig:L54i_is_same-as a owl:ObjectProperty;
    rdfs:domain crm:E1_CRM_Entity;
    rdfs:comment """This property describes the association kind of \"same as\" between objects. It is used to declare that two or more objects are
exactly the same."""@en;
    rdfs:range crm:E1_CRM_Entity .
  
  crmdig:L60_documents a owl:ObjectProperty;
    rdfs:domain crmdig:D2_Digitization_Process;
    rdfs:comment """This property describes the CRM Entities documented by instances of Digitization Processes.
This property is a specialisation of P140 assigned attribute to."""@en;
    rdfs:subPropertyOf crm:P140_assigned_attribute_to;
    rdfs:range crm:E1_CRM_Entity .
  
  crmdig:L56_has_pixel_width a owl:DatatypeProperty;
    rdfs:domain crmdig:D9_Data_Object;
    rdfs:subPropertyOf crm:P90_has_value;
    rdfs:comment """This property records the pixel width of the data object; it approximates a dimension that is 
part of the image data analysis.This property is a specialisation of P90 has value."""@en;
    rdfs:range xsd:string .
  
  crmdig:L59_has_serial_number a owl:DatatypeProperty;
    rdfs:domain crm:E22_Man-Made_Object;
    rdfs:range xsd:string;
    rdfs:subPropertyOf crmdig:L53_is_not_uniquely_identified_by;
    rdfs:comment """This property records the serial number that was assigned to identify an instance of E22 Man Made Object.
 This property is a specialisation of L53 is not uniquely identified by."""@en .
  
  crmdig:L61_was_ongoing_at a owl:ObjectProperty;
    rdfs:comment """This property describes the minimum period of time covered by a digital machine event. It 
identifies the minimum extent of the event. This property is a specialisation of P81 ongoing throughout."""@en;
    rdfs:domain crm:E5_Event;
    rdfs:subPropertyOf crm:P81a_end_of_the_begin, crm:P81b_begin_of_the_end;
    rdfs:range xsd:dateTime .
  
  crmdig:L49i_has_primary_area a owl:ObjectProperty;
    rdfs:range crmdig:D35_Area;
    rdfs:subPropertyOf crm:P106_is_composed_of;
    rdfs:domain crmdig:D1_Digital_Object .
  
  crmdig:L52_has_last_name a owl:DatatypeProperty;
    rdfs:range xsd:string;
    rdfs:subPropertyOf crmdig:L4_has_preferred_label;
    rdfs:domain crmdig:D21_Person_Name;
    rdfs:comment """This property defines the last name used to identify a person.
This property is a specialisation of L4 has preferred label."""@en .
  
  crmdig:L50_is_propagated_area_of a owl:ObjectProperty;
    rdfs:range crmdig:D1_Digital_Object;
    rdfs:domain crmdig:D35_Area;
    rdfs:comment """This property describes the association between an area and the digital object to which it is propagated.
This property is a specialisation of P106 is composed of."""@en;
    rdfs:subPropertyOf crm:P106i_forms_part_of .
  
  crmdig:L55_has_inventory_no a owl:DatatypeProperty;
    rdfs:range xsd:string;
    rdfs:subPropertyOf crmdig:L53_is_not_uniquely_identified_by;
    rdfs:comment """This property records the inventory number that was used to identify an instance of E1 CRM Entity 
at the time this property was record. This property is a specialisation of L53F is not uniquely identified by."""@en;
    rdfs:domain crm:E1_CRM_Entity .
  
  crmdig:L60i_is_documented_by a owl:ObjectProperty;
    rdfs:range crmdig:D2_Digitization_Process;
    rdfs:subPropertyOf crm:P140i_was_attributed_by;
    rdfs:domain crm:E1_CRM_Entity .
  
  crmdig:L57_has_pixel_height a owl:DatatypeProperty;
    rdfs:comment """This property records the pixel height of the data object; it approximates a dimension that is 
part of the image data analysis.This property is a specialisation of P90 has value."""@en;
    rdfs:range xsd:string;
    rdfs:subPropertyOf crm:P90_has_value;
    rdfs:domain crmdig:D9_Data_Object .
  
  crmdig:L54_is_same-as a owl:ObjectProperty;
    rdfs:comment """This property describes the association kind of \"same as\" between objects. It is used to declare that two or more objects are
exactly the same."""@en;
    rdfs:domain crm:E1_CRM_Entity;
    rdfs:range crm:E1_CRM_Entity .
  
  crmdig:L53_is_not_uniquely_identified_by a owl:DatatypeProperty;
    rdfs:comment "This property describes a non unique identification applied to E1 CRM Entity."@en;
    rdfs:domain crm:E1_CRM_Entity;
    rdfs:subPropertyOf rdfs:label;
    rdfs:range xsd:string .
  
  crmdig:L22_created_derivative a owl:ObjectProperty;
    rdfs:range crmdig:D1_Digital_Object;
    rdfs:comment """This property associates an instance of D3 Formal Derivation with the Digital Object it used to create a version of.
This property is a specialisation of L11 had output."""@en;
    rdfs:subPropertyOf crmdig:L11_had_output;
    rdfs:domain crmdig:D3_Formal_Derivation .
  
  crmdig:L19_stores a owl:ObjectProperty;
    rdfs:range crmdig:D1_Digital_Object;
    rdfs:subPropertyOf crm:P128_carries;
    rdfs:domain crmdig:D13_Digital_Information_Carrier;
    rdfs:comment """This property associates an instance of a D13 Digital Information Carrier with the instance of Digital Object 
that is stored on it. This property is a specialisation of P128 carries."""@en .
  
  crmdig:L17_measured_thing_of_type a owl:ObjectProperty;
    rdfs:domain crmdig:D11_Digital_Measurement_Event;
    rdfs:subPropertyOf crm:P125_used_object_of_type;
    rdfs:range crm:E55_Type;
    rdfs:comment """This property associates an instance of D11 Digital Measurement Event with the instance of E55
Type of object to which it applied. This property is a specialisation of P125 used object of type. """@en .
  
  crmdig:L18i_was_modified_by a owl:ObjectProperty;
    rdfs:subPropertyOf crm:P31i_was_modified_by;
    rdfs:range crmdig:D7_Digital_Machine_Event;
    rdfs:domain crmdig:D13_Digital_Information_Carrier .
  
  crmdig:L20_has_created a owl:ObjectProperty;
    rdfs:domain crmdig:D11_Digital_Measurement_Event;
    rdfs:range crmdig:D9_Data_Object;
    rdfs:subPropertyOf crm:P40_observed_dimension, crmdig:L11_had_output;
    rdfs:comment """This property identifies a Data Object that came into existence as a result of a D11 Digital Measurement Event.
This property is a specialisation of P40 observed dimension and L11 had output."""@en .
  
  crmdig:L16_has_receiver a owl:ObjectProperty;
    rdfs:comment """This property  identifies a digital device used as a medium to receive data  
through a D12 Data Transfer Event."""@en;
    rdfs:subPropertyOf crmdig:L12_happened_on_device;
    rdfs:domain crmdig:D12_Data_Transfer_Event;
    rdfs:range crmdig:D8_Digital_Device .
  
  crmdig:L14i_was_transferred_by a owl:ObjectProperty;
    rdfs:range crmdig:D12_Data_Transfer_Event;
    rdfs:subPropertyOf crmdig:L11i_was_output_of, crmdig:L10i_was_input_of;
    rdfs:domain crmdig:D1_Digital_Object .
  
  crmdig:L17i_was_type_of_thing_measured_by a owl:ObjectProperty;
    rdfs:subPropertyOf crm:P125i_was_type_of_object_used_in;
    rdfs:range crmdig:D11_Digital_Measurement_Event;
    rdfs:domain crm:E55_Type .
  
  crmdig:L20i_was_created_by a owl:ObjectProperty;
    rdfs:range crmdig:D11_Digital_Measurement_Event;
    rdfs:subPropertyOf crmdig:L11i_was_output_of, crm:P40i_was_observed_in;
    rdfs:domain crmdig:D9_Data_Object .
  
  crmdig:L18_has_modified a owl:ObjectProperty;
    rdfs:domain crmdig:D7_Digital_Machine_Event;
    rdfs:subPropertyOf crm:P31_has_modified;
    rdfs:comment """This property identifies a Digital Information Carrier modified in a Digital Machine Event.
This property is a specialisation of P31 has modified."""@en;
    rdfs:range crmdig:D13_Digital_Information_Carrier .
  
  crmdig:L2_used_as_source a owl:ObjectProperty;
    rdfs:comment """This property associates an instance of D10 Software Execution with an instance of D1 Digital Object
 which is used as a source, a software essential for the performance.  
This property is a specialisation of L10F had input (was input of).
	"""@en;
    rdfs:range crmdig:D1_Digital_Object;
    rdfs:subPropertyOf crmdig:L10_had_input;
    rdfs:domain crmdig:D10_Software_Execution .
  
  crmdig:L15i_was_sender_for a owl:ObjectProperty;
    rdfs:subPropertyOf crmdig:L12i_was_device_for;
    rdfs:domain crmdig:D8_Digital_Device;
    rdfs:range crmdig:D12_Data_Transfer_Event .
  
  crmdig:L16i_was_receiver_for a owl:ObjectProperty;
    rdfs:domain crmdig:D8_Digital_Device;
    rdfs:range crmdig:D12_Data_Transfer_Event;
    rdfs:subPropertyOf crmdig:L12i_was_device_for .
  
  crmdig:L21_used_as_derivation_source a owl:ObjectProperty;
    rdfs:comment "This property associates an instance of a D3 Formal Derivation with the instance of D1 Digital Object that is used as a derivation source."@en;
    rdfs:range crmdig:D1_Digital_Object;
    rdfs:domain crmdig:D3_Formal_Derivation;
    rdfs:subPropertyOf crmdig:L2_used_as_source .
  
  crmdig:L15_has_sender a owl:ObjectProperty;
    rdfs:comment """This property  identifies a digital device used as a medium on which data are transferred 
through a D12 Data Transfer Event."""@en;
    rdfs:subPropertyOf crmdig:L12_happened_on_device;
    rdfs:domain crmdig:D12_Data_Transfer_Event;
    rdfs:range crmdig:D8_Digital_Device .
  
  crmdig:L1i_was_digitized_by a owl:ObjectProperty;
    rdfs:subPropertyOf crm:P39i_was_measured_by;
    rdfs:domain crm:E18_Physical_Thing;
    rdfs:range crmdig:D2_Digitization_Process .
  
  crmdig:L14_transferred a owl:ObjectProperty;
    rdfs:range crmdig:D1_Digital_Object;
    rdfs:subPropertyOf crmdig:L10_had_input, crmdig:L11_had_output;
    rdfs:comment """This property  identifies a digital object transferred by a D12 Data Transfer Event.
This property is a specialisation of L11 had output (was output of)."""@en;
    rdfs:domain crmdig:D12_Data_Transfer_Event .
  
  crmdig:L21i_was_derivation_source_for a owl:ObjectProperty;
    rdfs:subPropertyOf crmdig:L2i_was_source_for;
    rdfs:range crmdig:D3_Formal_Derivation;
    rdfs:domain crmdig:D1_Digital_Object .
  
  crmdig:L22i_was_derivative_created_by a owl:ObjectProperty;
    rdfs:range crmdig:D3_Formal_Derivation;
    rdfs:domain crmdig:D1_Digital_Object;
    rdfs:subPropertyOf crmdig:L11i_was_output_of .
  
  crmdig:L19i_is_stored_on a owl:ObjectProperty;
    rdfs:domain crmdig:D1_Digital_Object;
    rdfs:subPropertyOf crm:P128i_is_carried_by;
    rdfs:range crmdig:D13_Digital_Information_Carrier .
}
