@prefix rs: <http://www.researchspace.org/ontology/> .
@prefix User: <http://www.researchspace.org/resource/user/> .
@prefix Help: <http://help.researchspace.org/resource/> .
@prefix Platform: <http://www.researchspace.org/resource/system/> .
@prefix owl: <http://www.w3.org/2002/07/owl#> .
@prefix xsd: <http://www.w3.org/2001/XMLSchema#> .
@prefix skos: <http://www.w3.org/2004/02/skos/core#> .
@prefix rdfs: <http://www.w3.org/2000/01/rdf-schema#> .
@prefix crmdig: <http://www.cidoc-crm.org/extensions/crmdig/> .
@prefix rsp: <http://www.researchspace.org/resource/> .
@prefix rshelp: <http://researchspace.org/help/> .
@prefix crmsci: <http://www.cidoc-crm.org/extensions/crmsci/> .
@prefix crmgeo: <http://www.cidoc-crm.org/extensions/crmgeo/> .
@prefix sp: <http://spinrdf.org/sp#> .
@prefix prov: <http://www.w3.org/ns/prov#> .
@prefix crminfluence: <http://www.cidoc-crm.org/extensions/influence/> .
@prefix crm: <http://www.cidoc-crm.org/cidoc-crm/> .
@prefix crminf: <http://www.cidoc-crm.org/extensions/crminf/> .
@prefix Admin: <http://www.researchspace.org/resource/admin/> .
@prefix bds: <http://www.bigdata.com/rdf/search#> .
@prefix rdf: <http://www.w3.org/1999/02/22-rdf-syntax-ns#> .
@prefix crmba: <http://www.cidoc-crm.org/extensions/crmba/> .
@prefix ontodia: <http://ontodia.org/schema/v1#> .
@prefix crmarchaeo: <http://www.cidoc-crm.org/extensions/crmarchaeo/> .
@prefix forms: <http://www.researchspace.org/resource/system/forms/> .
@prefix lrmoo: <http://iflastandards.info/ns/lrm/lrmoo/> .
@prefix crmtex: <http://www.cidoc-crm.org/extensions/crmtex/> .

crmba:context {

  <http://www.cidoc-crm.org/extensions/crmba/> a owl:Ontology;
    rdfs:label "CRMba v1.4"@en;
    owl:versionInfo "1.4"@en;
    rdfs:comment "The CRMba is an ontology to encode metadata about the documentation of archaeological buildings. The model was conceived to support the process of recording the evidences and the discontinuities of matter on archaeological buildings, in order to identify the evolution of the structure throughout the centuries and to record the relationships between each of the building components among them and with the building as a whole."@en .
    
  crmba:B1_Built_Work a owl:Class;
    skos:prefLabel "B1 Built Work"@en ;
    skos:notation "B1" ;
    rdfs:label "Built Work"@en;
    rdfs:subClassOf crm:E24_Physical_Human-Made_Thing, crm:E92_Spacetime_Volume;
    rdfs:comment """This class comprises instances of human-made things such as freestanding buildings, components of buildings, 
    and complexes of buildings. It refers to human-made environments, typically large enough for humans to enter, serving a 
    practical purpose, being relatively permanent and stable. Instances of built works are composed of parts that share an aspect of role, which often perform a distinct function."""@en ;
    skos:example """- The Bishop’s Palace \n
    - The ruins of Loropéni \n
    - The Coliseum"""@en.
  
  crmba:B2_Morphological_Building_Section a owl:Class;
    skos:prefLabel "B2 Morphological Building Section"@en ;
    skos:notation "B2" ;
    rdfs:label "Morphological Building Section"@en;
    rdfs:subClassOf crmba:B1_Built_Work;
    rdfs:comment """This class comprises instances of human-made things that are considered functional units for the whole building 
    (e.g. rooms, foundations, roof, and so forth). A Morphological Building Section is a geometric feature with volume and is a Spacetime Volume. 
    A Morphological Building Section is composed of parts that are completely filled with matter (Filled Morphological Building Section), 
    and of empty spaces (Empty Morphological Building Section) that are the result of the intentional disposition of a set of Filled Morphological Building Section."""@en;
    skos:example """- The western wall of the Cathedral \n
    - The corner tower \n
    - The battlements of the palace perimeter"""@en.

  crmba:B3_Filled_Morphological_Building_Section a owl:Class;
    rdfs:subClassOf crm:E24_Physical_Human-Made_Thing, crmba:B2_Morphological_Building_Section;
    skos:prefLabel "B3 Filled Morphological Building Section"@en ;
    skos:notation "B3" ;
    rdfs:label "Filled Morphological Building Section"@en ;
    rdfs:comment """This class comprises instances of human-made things that are completely filled with matter. Instances of 
    Filled Morphological Building Section are components of the functional units of a built work. These elements like walls, 
    floors and ceilings have properties such as dimensions, material etc. The intentional disposition of a set of Filled Morphological Building Section defines 
    portions of space that are completely void, e.g. a window, a doorway and so forth."""@en;
    skos:example """- The ionic columns of the portico \n
    - The walls that surround a room"""@en.

  crmba:B4_Empty_Morphological_Building_Section a owl:Class;
    skos:prefLabel "B4 Empty Morphological Building Section"@en ;
    skos:notation "B4" ;
    rdfs:label "Empty Morphological Building Section"@en ;
    rdfs:subClassOf crmsci:S20_Rigid_Physical_Feature;
    rdfs:comment """This class comprises identifiable features that are physically attached to particular physical objects. 
    Instances of Empty Morphological Building Section are components of the functional units that for a built work. 
    Example are the empty spaces that are formed by their surrounding walls, floors and ceiling. Empty spaces are fundamental 
    elements in modeling environments like BIM that need to have explicit space objects where the spaces are formed by the 
    surrounding objects (Underwood et al. 2009). Instances of B4 are portions of the space resulting from the intentional 
    disposition in the space of a set of Filled Morphological Building Sections. The void space must be intentionally obtained to serve a function for the building.
    """@en;
    skos:example """Examples of B4 are the empty spaces that are formed by their surrounding walls, floors and ceiling. Empty spaces are fundamental elements in modelling environments like BIM that need to have explicit space objects where the spaces are formed by the surrounding objects (Underwood et al. 2009). Instances of B4 are portions of the space resulting from the intentional disposition in the space of a set of Filled Morphological Building Sections. The void space must be intentionally obtained to serve a function for the building.The intercolumniation of a portico. \n
    - The Gate of Felicity of Topkapı Palace \n
    - The compluvium of the roof of a Roman Domus \n
    - The portico of the Temple of Ercole Vincitore (B1) is composed of columns (B3)  \n
    - that confine (AP12) the intercolumniation (B4)"""@en.
    
  crmba:B5_Stratigraphic_Building_Unit a owl:Class;
    skos:prefLabel "B5 Stratigraphic Building Unit"@en ;
    skos:notation "B5" ;
    rdfs:label "Stratigraphic Building Unit"@en ;
    rdfs:subClassOf crmarchaeo:A2_Stratigraphic_Volume_Unit;
    rdfs:comment """This class comprises instances of physical things that represents the minimal construction unit of a built work. The Stratigraphic Building Unit 
    is a constituent part of a Morphological Building Section. The Stratigraphic Building Unit represents a single evidence of human activity intentionally 
    performed on the building: e.g. the presence of mortar, vestments or any of the discontinuities of matter that can be observed on a wall surface. 
    The term constituency is used within the model with the meaning: “the status of being a constituent part”.
    Instances of Stratigraphic Building Unit are, for example, a single wall or the various architectonic components that constitute the Morphologic Building Section. 
    """@en;
    skos:example """- The fresco decoration of the great hall"""@en.

  crmba:BP1_is_section_of a owl:ObjectProperty;
    skos:prefLabel "BP1 is section of"@en ;
    skos:notation "BP1" ;
    rdfs:label "is section of"@en;
    rdfs:domain crmba:B2_Morphological_Building_Section;
    rdfs:range crmba:B1_Built_Work;
    owl:inverseOf crmba:BP1i_has_section ;
    rdfs:comment """This property is used to link the Morphological Building Sections that are part of a Built Work.
    
    Examples:
    - The great hall (BP1 is section of) the Bishop’s Palace"""@en;
    skos:example """- The great hall (BP1 is section of) the Bishop’s Palace"""@en.
  
  crmba:BP1i_has_section a owl:ObjectProperty;
    skos:prefLabel "BP1i has section"@en ;
    skos:notation "BP1i" ;
    rdfs:label "has section"@en;
    rdfs:range crmba:B2_Morphological_Building_Section;
    rdfs:domain crmba:B1_Built_Work ;
    owl:inverseOf crmba:BP1_is_section_of ;
    rdfs:comment """This property is used to link the Morphological Building Sections that are part of a Built Work.

    Examples:
    - The great hall (BP1 is section of) the Bishop’s Palace"""@en;
    skos:example """- The great hall (BP1 is section of) the Bishop’s Palace"""@en.

  crmba:BP2_is_constituent_of a owl:ObjectProperty;
    skos:prefLabel "BP2 is constituent of"@en ;
    skos:notation "BP2" ;
    rdfs:label "is constituent of"@en;
    rdfs:range crmba:B1_Built_Work;
    rdfs:domain crmba:B5_Stratigraphic_Building_Unit ;
    owl:inverseOf crmba:BP2i_is_constituted_by ;
    rdfs:comment """This property describes the relation between a Morphological Building Section (e.g. a wall) and any Stratigraphic Building Section. 
    When the SBU and the MBS are equal we can use the shortcut: SBU (is constituent of) Built Work.

    Examples:
    - The fresco of the great hall (BP2 is constituent of) the northern wall"""@en;
    skos:example """- The fresco of the great hall (BP2 is constituent of) the northern wall"""@en.
  
  crmba:BP2i_is_constituted_by a owl:ObjectProperty;
    skos:prefLabel "BP2i is constituted by"@en ;
    skos:notation "BP2i" ;
    rdfs:label "is constituted by"@en;
    rdfs:domain crmba:B1_Built_Work;
    rdfs:range crmba:B5_Stratigraphic_Building_Unit ;
    owl:inverseOf crmba:BP2_is_constituent_of ;
    rdfs:comment """This property describes the relation between a Morphological Building Section (e.g. a wall) and any Stratigraphic Building Section. 
    When the SBU and the MBS are equal we can use the shortcut: SBU (is constituent of) Built Work.

    Examples:
    - The fresco of the great hall (BP2 is constituent of) the northern wall"""@en;
    skos:example """- The fresco of the great hall (BP2 is constituent of) the northern wall"""@en.

  crmba:BP3_is_spatial_temporary_equal_to a owl:ObjectProperty;
    skos:prefLabel "BP3 is spatial temporary equal to"@en ;
    skos:notation "BP3" ;
    rdfs:label "is spatial temporary equal to"@en;
    rdfs:domain crm:E92_Spacetime_Volume;
    rdfs:range crm:E92_Spacetime_Volume;
    rdfs:comment """This property is used to relate the Spacetime Volume of two entities (Morphological Building Units and Stratigraphic Building Section). 
    When the two STV overlap, the two entities are equal.
    
    Examples:
    - The STV of the plaster that completely covers the wall surface (BP3 is spatial temporary equal to) the STV of the masonry"""@en ;
    skos:example """- The STV of the plaster that completely covers the wall surface (BP3 is spatial temporary equal to) the STV of the masonry"""@en.
  
  crmba:BP4_terminates_the_constituency a owl:ObjectProperty;
    skos:prefLabel "BP4 terminates the constituency"@en ;
    skos:notation "BP4" ;
    rdfs:label "terminates the constituency"@en;
    rdfs:range crmba:B2_Morphological_Building_Section;
    rdfs:domain crm:E80_Part_Removal;
    owl:inverseOf  crmba:BP4i_constituency_was_terminated_by;
    rdfs:comment """This property is used to describe the constituency (being part of) of a Stratigraphic Building Section with a 
    Filled Morphological Building Section. The constituency ends when an entity (FMBS) is diminished by matter.
    
    Examples:
    - The removal of the fresco from the northern wall (BP4 terminates the constituency) of the fresco to the wall"""@en ;
    skos:example """- The removal of the fresco from the northern wall (BP4 terminates the constituency) of the fresco to the wall"""@en.
  
  crmba:BP4i_constituency_was_terminated_by a owl:ObjectProperty;
    skos:prefLabel "BP4i constituency was terminated by"@en ;
    skos:notation "BP4i" ;
    rdfs:label "constituency was terminated by"@en;
    rdfs:range crm:E80_Part_Removal;
    rdfs:domain crmba:B2_Morphological_Building_Section ;
    owl:inverseOf crmba:BP4_terminates_the_constituency;
    rdfs:comment """This property is used to describe the constituency (being part of) of a Stratigraphic Building Section with a 
    Filled Morphological Building Section. The constituency ends when an entity (FMBS) is diminished by matter.
    
    Examples:
    - The removal of the fresco from the northern wall (BP4 terminates the constituency) of the fresco to the wall"""@en ;
    skos:example """- The removal of the fresco from the northern wall (BP4 terminates the constituency) of the fresco to the wall"""@en.
    
  crmba:BP5_initiates_the_constituency a owl:ObjectProperty;
    skos:prefLabel "BP5 initiates the constituency"@en ;
    skos:notation "BP5" ;
    rdfs:label "initiates the constituency"@en;
    owl:inverseOf crmba:BP5i_constituency_was_initiated_by ;
    rdfs:range crmba:B2_Morphological_Building_Section;
    rdfs:domain crm:E79_Part_Addition ;
    rdfs:comment """This property is used to describe the beginning of the constituency of a Stratigraphic Building Unit 
    with a Morphological Building Section. This starts when substance is added to a Morphological Building Unit. 
    
    Examples:
    - The painting of the fresco on the northern wall (BP5 initiates the constituency) of the painting to the wall
    """@en;
    skos:example """- The painting of the fresco on the northern wall (BP5 initiates the constituency) of the painting to the wall"""@en.

  crmba:BP5i_constituency_was_initiated_by a owl:ObjectProperty;
    skos:prefLabel "BP5i constituency was initiated by"@en ;
    skos:notation "BP5i" ;
    rdfs:label "constituency was initiated by"@en;
    owl:inverseOf crmba:BP5_initiates_the_constituency ;
    rdfs:domain crmba:B2_Morphological_Building_Section;
    rdfs:range crm:E79_Part_Addition ;
    rdfs:comment """This property is used to describe the beginning of the constituency of a Stratigraphic Building Unit 
    with a Morphological Building Section. This starts when substance is added to a Morphological Building Unit. 

    Examples:
    - The painting of the fresco on the northern wall (BP5 initiates the constituency) of the painting to the wall"""@en;
    skos:example """- The painting of the fresco on the northern wall (BP5 initiates the constituency) of the painting to the wall"""@en.

  crmba:BP11_is_connected_to a owl:ObjectProperty ;
    skos:prefLabel "BP11 is connected to"@en ;
    skos:notation "BP11" ;
    rdfs:label "is connected to"@en ;
    rdfs:domain crmba:B2_Morphological_Building_Section ;
    rdfs:range crmba:B2_Morphological_Building_Section ;
    rdfs:comment """This property identifies the instance of Morphological Building Section which is connected to another instance of 
    Morphological Building Section. The instance of Physical Man Made Thing through which the connection between the two 
    instances of Morphological Building Section is made, can be recorded using the property BP11.2 is connected through.
    
    Examples:
    - The great hall (B2) is connected to the sacristy (B2)"""@en;
    skos:example """- The great hall (B2) is connected to the sacristy (B2)"""@en.

  crmba:BP13_used_specific_object a owl:ObjectProperty;
    skos:prefLabel "BP13 used specific object"@en ;
    skos:notation "BP13" ;
    rdfs:label "used specific object"@en ;
    owl:inverseOf crmba:BP13i_was_specific_object_used_by;
    rdfs:domain crm:E12_Production;
    rdfs:range crmba:B5_Stratigraphic_Building_Unit;
    rdfs:comment """This property is used to describe an instance of a physical object that is used in the production of new substance 
    that constitutes the Morphological Building Section (i.e. a Stratigraphic Building Section).
    
    Examples:
    - The construction of the new façade (BP13 used specific object) the staircase"""@en;
    skos:example """- The construction of the new façade (BP13 used specific object) the staircase"""@en.

  crmba:BP13i_was_specific_object_used_by a owl:ObjectProperty;
    skos:prefLabel "BP13i was specific object used by"@en ;
    skos:notation "BP13i" ;
    rdfs:label "was specific object used by"@en ;
    owl:inverseOf crmba:BP13_used_specific_object;
    rdfs:domain crmba:B5_Stratigraphic_Building_Unit;
    rdfs:range crm:E12_Production;
    rdfs:comment """This property is used to describe an instance of a physical object that is used in the production of new substance 
    that constitutes the Morphological Building Section (i.e. a Stratigraphic Building Section).
    
    Examples:
    - The construction of the new façade (BP13 used specific object) the staircase"""@en;
    skos:example """- The construction of the new façade (BP13 used specific object) the staircase"""@en.
     
  crmba:BP14_re-used_specific_object a owl:ObjectProperty;
    skos:prefLabel "BP14 re-used specific object"@en ;
    skos:notation "BP14" ;
    rdfs:label "re-used specific object"@en;
    owl:inverseOf crmba:BP14i_was_specific_object_re-used_by ;
    rdfs:range crmba:B5_Stratigraphic_Building_Unit;
    rdfs:domain crm:E12_Production ;
    rdfs:comment """This property is used to describe an instance of a physical object that is re-used in the production 
    of new substance that constitutes the Morphological Building Section (i.e. a Stratigraphic Building Section).
    
    Examples:
    - The stones of the Roman theatre (BP14 was specific object re-used by) the construction of the fountain"""@en;
    skos:example """- The stones of the Roman theatre (BP14 was specific object re-used by) the construction of the fountain"""@en.

  crmba:BP14i_was_specific_object_re-used_by a owl:ObjectProperty;
    skos:prefLabel "BP14i was specific object re-used by"@en ;
    skos:notation "BP14i" ;
    rdfs:label "was specific object re-used by"@en;
    owl:inverseOf crmba:BP14_re-used_specific_object ;
    rdfs:range crm:E12_Production;
    rdfs:domain crmba:B5_Stratigraphic_Building_Unit ;
    rdfs:comment """This property is used to describe an instance of a physical object that is re-used in the production 
    of new substance that constitutes the Morphological Building Section (i.e. a Stratigraphic Building Section).
    
    Examples:
    - The stones of the Roman theatre (BP14 was specific object re-used by) the construction of the fountain"""@en;
    skos:example """- The stones of the Roman theatre (BP14 was specific object re-used by) the construction of the fountain"""@en .

  crmba:BP15_is_equal_to a owl:ObjectProperty;
    skos:prefLabel "BP15 is equal to"@en ;
    skos:notation "BP15" ;
    rdfs:label "is equal to"@en;
    rdfs:domain crmba:B5_Stratigraphic_Building_Unit;
    rdfs:range crmba:B3_Filled_Morphological_Building_Section;
    rdfs:comment """This property is used to relate a Stratigraphic Building Section with a Morphological Building Section when the former is equal to the latter. 
    
    Examples:
    - The northern wall (BP 15 is equal to) the SBU “northern wall"""@en ;
    skos:example """- The northern wall (BP 15 is equal to) the SBU “northern wall"""@en .
}
