@prefix rs: <http://www.researchspace.org/ontology/> .
@prefix User: <http://www.researchspace.org/resource/user/> .
@prefix Help: <http://help.researchspace.org/resource/> .
@prefix Platform: <http://www.researchspace.org/resource/system/> .
@prefix owl: <http://www.w3.org/2002/07/owl#> .
@prefix xsd: <http://www.w3.org/2001/XMLSchema#> .
@prefix skos: <http://www.w3.org/2004/02/skos/core#> .
@prefix rdfs: <http://www.w3.org/2000/01/rdf-schema#> .
@prefix crmdig: <http://www.cidoc-crm.org/extensions/crmdig/> .
@prefix rshelp: <http://researchspace.org/help/> .
@prefix crmsci: <http://www.cidoc-crm.org/extensions/crmsci/> .
@prefix assets: <http://www.researchspace.org/resource/assets/> .
@prefix crmgeo: <http://www.cidoc-crm.org/extensions/crmgeo/> .
@prefix sp: <http://spinrdf.org/sp#> .
@prefix prov: <http://www.w3.org/ns/prov#> .
@prefix crminfluence: <http://www.cidoc-crm.org/extensions/influence/> .
@prefix crm: <http://www.cidoc-crm.org/cidoc-crm/> .
@prefix crminf: <http://www.cidoc-crm.org/extensions/crminf/> .
@prefix Admin: <http://www.researchspace.org/resource/admin/> .
@prefix bds: <http://www.bigdata.com/rdf/search#> .
@prefix rdf: <http://www.w3.org/1999/02/22-rdf-syntax-ns#> .
@prefix crmba: <http://www.cidoc-crm.org/extensions/crmba/> .
@prefix fedsail: <http://www.openrdf.org/config/sail/federation#> .
@prefix ontodia: <http://ontodia.org/schema/v1#> .
@prefix crmarchaeo: <http://www.cidoc-crm.org/extensions/crmarchaeo/> .
@prefix forms: <http://www.researchspace.org/resource/system/forms/> .
@prefix lrmoo: <http://iflastandards.info/ns/lrm/lrmoo/> .
@prefix crmtex: <http://www.cidoc-crm.org/extensions/crmtex/> .

crmtex:context {

  <http://www.cidoc-crm.org/extensions/crmtex/> a owl:Ontology ;
    owl:versionInfo "2.0"@en;
    rdfs:label "CRMtex v2.0"@en ;
    rdfs:comment """CRMtex is a formal ontology intended to support the study of ancient documents by identifying relevant textual entities and 
    by modelling the scientific process related with the investigation of ancient texts and their features in order to foster integration with other 
    cultural heritage research fields, such as archaeology and history. 
    The concept of “written text”, introduced by the ontology, is intended to identify a common entity consisting in a particular 
    feature (i.e., set of glyphs) created (i.e., written) on various kinds of support, having semiotic significance and the declared purpose of 
    conveying a specific message towards a given recipient or group of recipients. The modelling of the scientific autoptic examination of the document, consisting of an 
    accurate analysis of the surface and the signs and prescribing the use of specific tools and procedures, is another key aspect taken into account by this ontology.""".

  crmtex:TX1_Written_Text
    a owl:Class ;
    skos:prefLabel "TX1 Written Text"@en ;
    skos:notation "TX1" ;
    rdfs:label "Written Text"@en ;
    rdfs:subClassOf crm:E25_Human-Made_Feature;
    rdfs:comment """This class comprises visible or tactile marks (called glyphs or graphs), which relate in a systematic way to units of speech, intentionally traced 
    (i.e., “written”) on some kind of physical support by using specific techniques and tools, with the purpose of conveying a message 
    towards a given receiver or group of receivers."""@en ;
    skos:example """- The signs composing the inscription engraved on the South side of the attic of the Arch of Constantine (Human-made object) in Rome \n
    - The signs composing the text written on papyrus PSI XIII 1304 containing the so-called Hellenica Oxyrhynchia (TM 59482)"""@en.

  crmtex:TX2_Writing
    a owl:Class ;
    skos:prefLabel "TX2 Writing"@en ;
    skos:notation "TX2" ;
    rdfs:label "Writing"@en ;
    rdfs:subClassOf lrmoo:F28_Expression_Creation ;
    rdfs:comment """This class describes the activity of communicating information by means of permanent, visible marks in a 
    non-mechanical way, using various techniques (painting, sculpture, etc.) and by means of specific tools, on a given support."""@en ;
    skos:example """- The process of engraving in the marble of the inscription (Written Text) placed on the south attic of the Arch of 
    Constantine (Human-made object) in Rome"""@en.

  crmtex:TX3_Writing_System
    a owl:Class ;
    skos:prefLabel "TX3 Writing System"@en ;
    skos:notation "TX3" ;
    rdfs:label "Writing System"@en ;
    rdfs:subClassOf crm:E29_Design_or_Procedure;
    rdfs:comment """This class represents a conventional symbolic system designed to represent units of a natural 
    language with the purpose of recording and transmitting information. A writing system consists of a set of
    symbols (graphemes), instantiated through physical signs of a visual or tactile nature (glyphs) representing 
    linguistic units of any kind and the related syntactic (i.e., graphotactic) rules.It is used to produce a Written Text during a Writing event."""@en ;
    skos:example """- The Latin alphabet used to encode the signs (Written Text) composing the text (Linguistic Object) of the inscription 
    in Latin language occurring on the Arch of Constantine (Human-made object) \n
    - The Roman Latin writing system for creating public inscriptions \n
    - The Cypriot syllabary used in Iron Age Cyprus for codifying the Arcado-Cypriot dialect \n
    - The Chinese (Han) script used by Wang Xizhi to write the manuscript Lanting Xu (“Orchid Pavilion Preface”)"""@en.

  crmtex:TX4_Writing_Field
    a owl:Class ;
    skos:prefLabel "TX4 Writing Field"@en ;
    skos:notation "TX4" ;
    rdfs:label "Writing Field"@en ;
    rdfs:subClassOf crm:E25_Human-Made_Feature;
    rdfs:comment """This class describes the portion of the physical carrier arranged and usually reserved and delimited 
    for the purpose of accommodating a written text, highlighting and isolating it from the other 
    parts of the object to which it belongs, enhancing and guaranteeing its readability. This entity is 
    paramount specially in epigraphy, in which a specific element called “epigraphic field” has been defined 
    by the discipline itself. Its importance is also evident in papyrology and codicology, where a clear 
    distinction between area(s) containing the written text and empty parts of the support (margins, intercolumnia, etc.) 
    is significant for the definition of styles and periods of the document."""@en ;
    skos:example """- The portion of the marble tombstone (Human-made object) of M. Helvius Geminus from Ephesus reserved 
    for accommodating the inscription (Written Text)"""@en.

  crmtex:TX5_Text_Recognition
    a owl:Class ;
    skos:prefLabel "TX5 Text Recognition"@en ;
    skos:notation "TX5" ;
    rdfs:label "Text Recognition"@en ;
    rdfs:subClassOf crm:E65_Creation, crmsci:S4_Single_Observation;
    rdfs:comment """This class comprises activities of recognizing physical features on some surface, often an 
    instance of Writing Field, as an arrangement of a series of identifiable glyphs of some known script, 
    deciphered or not, in an order characteristic for a text.
    For study purposes, the text recognition procedure requires a scientific autoptic examination of the text. 
    An autoptic examination consists of an accurate analysis of the surface and the signs, and prescribes the 
    use of specific tools and procedures for establishing the exact value of each sign on the physical feature. 
    Deterioration of the original medium or “sloppy” writing may render parts of the original text as 
    undecipherable or ambiguous, which may be annotated in the transcript following epigraphic standards; 
    a text recognition typically results in a record of an equivalent sequence of graphemes on another 
    persistent medium in a scholarly established form of representation of the respective graphemes, 
    often called a “transcript”.
    An instance of Text Recognition may in particular apply even to a single glyph, typically forming 
    part of an instance of Text Recognition applying to a larger sequence of glyphs containing the former glyph.
    The recognition process may be assisted by mechanical means, imaging technology, or a traditional 
    squeeze for incised glyphs. In case the recognition process is solely based on the latter, the 
    observation concerns only the representations on the latter as present to the researcher in 
    some physical form or projection and should unambiguously be documented as such.

    In case the recognized text has not been documented in a transcript, text recognition may constitute 
    an implicit part of an overarching reading process, instance of Reading, which has resulted in other 
    noteworthy propositions related to the content of the recognized text. On the other side, recognition of 
    single glyphs or contracted parts of texts, as they are characteristic for the use of ligatured scripts, 
    may quite well be implicitly supported by the reader’s comprehension of the text and the creator of 
    the transcript may have chosen not to annotate parts that the reader regarded as unambiguous. Since 
    these cases can often hardly be separated from the shape recognition of the glyphs in isolation, 
    documenting such implicit comprehension as a separate process may not be relevant. It is however 
    regarded as good practice to document explicitly the reading process and associated interpretative 
    reasoning for any non-trivial resolution of ambiguity or gaps in the recognized text that has a bearing 
    on the transcript or further completion of the transcript."""@en ;
    skos:example """- The autoptic investigation of the South inscription (Written Text) on the Arch of Constantine 
    (Human-made object) made by Rodolfo Lanciani between 1893 and 1901"""@en.

  crmtex:TX6_Transliteration
    a owl:Class ;
    skos:prefLabel "TX6 Transliteration"@en ;
    skos:notation "TX6" ;
    rdfs:label "Transliteration"@en ;
    rdfs:subClassOf crm:E65_Creation;
    rdfs:comment """This class comprises activities of exactly re-writing (i.e., re-encoding) an instance of Grapheme 
    Sequence, i.e., the characters of a text, a contiguous part or a single character of it, by using a writing system
    different from that of the original text, without changing the order of characters or words, by using standard correspondences.
    This operation may apply a 1:1 relation between the signs of the two writing systems, a “transliteration” in the narrower 
    sense (e.g., the ALA-LC Romanization of Greek to Latin). It may also apply an approximation of the sounds of a language, 
    as defined by the source writing system, by that of the target writing system, normally called a “transcription” 
    (e.g., the “rōmaji” Romanization of Japanese), or a mixture of both (e.g. the ELOT 743 Type 2 – transcription of 
    Greek to Latin letters). In a broader sense, the term “transcription” also applies to the activity of re-encoding 
    a text using the same writing system (see example 1). The P16 used specific object (was used for) property 
    can be used to specify the applied method of correspondence."""@en ;
    skos:example """- Transcription, in Latin letters, of the Latin inscription(s) (Written Text) on the Arch of Constantine 
    (Human-made object) reported in Corpus Inscriptionum Latinarum (CIL VI 1139) \n
    - The transliteration and the transcription of the ancient Persian name of king Darius I, written in Persian 
    cuneiform https://cidoc-crm.org/extensions/crmtex/html/xml-html/images_2.0/crmtex_img_011.png, into Latin script as 
    respectively ‘da-a-ra-ya-va-u-ša’ and ‘Dârayavauš’"""@en.

  crmtex:TX7_Written_Text_Segment
    a owl:Class ;
    skos:prefLabel "TX7 Written Text Segment"@en ;
    skos:notation "TX7" ;
    rdfs:label "Written Text Segment"@en ;
    rdfs:subClassOf crmtex:TX1_Written_Text;
    rdfs:comment """This class describes portions of text considered to be of particular significance by scholars, as witnesses 
    of a certain 
    meaning or bearers of a particular phenomenon relevant to the investigation, study and understanding of a text. 
    Examples of such text portions are columns, fragments, sections, paragraphs, as well as single words or signs, 
    or other components of a written text. To each of these entities can be associated a single production event or destruction event, 
    as in the case of letters or words damaged or worn by atmospheric agents or human interventions, as well as specific conditions 
    for documenting 
    its status during the text recognition process. The relationship between a written text and its components is documented 
    through the 'has segment' property."""@en ;
    skos:example """- The “INSTINCTV DIVINITATIS” text portion of the inscription (Written Text) on the Arch of Constantine 
    (Human-made object), commented by Rodolfo Lanciani in 1892, in his book Pagan and Christian Rome \n
    - The first paragraph of the Darius I’s inscription (Written Text) in Bagistan"""@en.

  crmtex:TX8_Grapheme
    a owl:Class ;
    skos:prefLabel "TX8 Grapheme"@en ;
    skos:notation "TX8" ;
    rdfs:label "Grapheme"@en ;
    rdfs:subClassOf crm:E55_Type;
    rdfs:comment """This class comprises symbols used as kinds of atomic units with distinctive value in a given writing system 
    in order to represent linguistic units of some level to encode elements of a message. According to the typology of the 
    writing system, the represented linguistic units can be phonemes (as in Latin), syllables (as in Mycenaean Linear B), 
    up to complete words (as in Chinese and Sumerian scripts).
    A writing system also provides the conventions determining how the graphemes are to be used to write a language (orthographic rules).
    In some writing systems, graphemes may also be used as auxiliary signs, for instance, for disambiguating senses of homonyms, as in 
    the Japanese writing system, or to mark the semantic categories of the words, as in the ancient Egyptian determinatives."""@en ;
    skos:example """- The abstract unit “S” of the Latin alphabet, used to represent the /s/ sound \n
    - The abstract unit https://cidoc-crm.org/extensions/crmtex/html/xml-html/images_2.0/crmtex_img_012.png of the ancient 
    Persian syllabary, used to represent the /da/ syllable \n
    - The abstract unit “安” of the Han script, used to represent the meaning “peace” \n
    - 行きます, ching, gyo, iku, zuku"""@en.

  crmtex:TX9_Glyph
    a owl:Class ;
    skos:prefLabel "TX9 Glyph"@en ;
    skos:notation "TX9" ;
    rdfs:label "Glyph"@en ;
    rdfs:subClassOf crmtex:TX7_Written_Text_Segment;
    rdfs:comment """This class describes the physical, concrete features traced by a writer, representing the material manifestations 
    of the graphemes 
    needed to codify a linguistic expression. Glyphs are typically observed by the scholars during a text recognition activity 
    carried out 
    to decode and recognise the graphemes they represent."""@en ;
    skos:example """- The S-shaped feature engraved on the second line of the South inscription on the Arch of Constantine, 
    representing the letter (grapheme) 
    “S” of the Latin writing system used to render the sound of the /s/ phoneme \n
    - The first feature engraved on the first line of Darius I’s inscription (Written Text) in Bagistan, representing the ideal 
    syllabogram https://cidoc-crm.org/extensions/crmtex/html/xml-html/images_2.0/crmtex_img_013.png of the ancient Persian syllabary, 
    used to render the /da/ syllable"""@en.

  crmtex:TX10_Style
    a owl:Class ;
    skos:prefLabel "TX10 Style"@en ;
    skos:notation "TX10" ;
    rdfs:label "Style"@en ;
    rdfs:subClassOf crm:E29_Design_or_Procedure;
    rdfs:comment """This class describes stylistic variations of texts, including local script styles (as the Carolingian minuscule for the Latin script) 
    and individual scribal hands. It includes: the general appearance of the script, in terms of general design, aspects related to a 
    bilinear system (i.e., upper- and lowercase), measures (i.e., large, medium or small), shape and number of strokes forming a character, 
    its order and direction. A style includes also information about ductus (the direction the text), ligatures and nexi (i.e., the connection 
    between characters obtained by tracing them without detaching the writing instrument from the support and using one or more strokes in common), 
    and the writing angle (i.e., the position the writing instrument is located with respect to the support). The style corresponds to fonts and 
    their variations in the modern printing process."""@en ;
    skos:example """- The Roman square capitals style, also called capitalis monumentalis, or capitalis quadrata used to write the inscription on the Arch of Constantine \n
    - The “Carolingian minuscule” style used in the Carolingian Gospel Book identified as “British Library, Add MS 11848”"""@en.

  crmtex:TX11_Grapheme_Occurrence
    a owl:Class ;
    skos:prefLabel "TX11 Grapheme Occurrence"@en ;
    skos:notation "TX11" ;
    rdfs:label "Grapheme Occurrence"@en ;
    rdfs:subClassOf crmtex:TX12_Grapheme_Sequence;
    rdfs:comment """This class comprises single occurrences of a Grapheme used as an atomic unit at a particular position in the abstract form of a 
    given particular piece of text."""@en ;
    skos:example """- The ideal letter “S” of the Latin alphabet, used to represent the /s/ sound, rendered by the specific S-shaped feature engraved 
    on the second line of the South inscription on the attic of the Arch of Constantine \n
    - The ideal ‘da’ syllabogram of the ancient Persian syllabary, used to represent the /da/ syllable rendered by the 
    cuneiform sign https://cidoc-crm.org/extensions/crmtex/html/xml-html/images_2.0/crmtex_img_014.png engraved on the first line of Darius I’s 
    inscription (Written Text) in Bagistan"""@en.

  crmtex:TX12_Grapheme_Sequence
    a owl:Class ;
    skos:prefLabel "TX12 Grapheme Sequence"@en ;
    skos:notation "TX12" ;
    rdfs:label "Grapheme Sequence"@en ;
    rdfs:subClassOf crm:E90_Symbolic_Object;
    rdfs:comment """This class comprises particular sequences of Graphemes used for representing the abstract written form of a section of a given particular text."""@en ;
    skos:example """- The grapheme sequence ‘INSTINCTV DIVINITATIS’ [as recognised by the autoptic investigation of the Arch of Constantine, carried out by Rodolfo Lanciani]"""@en.

  crmtex:TX13_Script
    a owl:Class ;
    skos:prefLabel "TX13 Script"@en ;
    skos:notation "TX13" ;
    rdfs:label "Script"@en ;
    rdfs:subClassOf crm:E89_Propositional_Object;
    rdfs:comment """This class comprises functionally complete sets of mutually different graphemes employed by one or more languages, regardless of the specific 
    operating rules in a particular language. A writing system, on the other hand, also refers to the set of relations between symbols and 
    linguistic units they represent. The same language may be written using different scripts."""@en ;
    skos:example """- The Latin script used by the Italian and English writing systems \n
    - The Latin and the Greek scripts used for the encoding of the Oscan language, creating the Oscan-Greek and Oscan-Latin writing systems"""@en.

  crmtex:TX14_Reading
    a owl:Class ;
    skos:prefLabel "TX14 Reading"@en ;
    skos:notation "TX14" ;
    rdfs:label "Reading"@en ;
    rdfs:subClassOf crminf:I1_Argumentation ;
    rdfs:comment """This class describes the complete intellectual activity, involving the interaction of visual-perceptual, linguistic, and 
    conceptual systems, leading from Text Recognition until its association with a complete linguistic meaning."""@en ;
    skos:example """- The reading of the South inscription (Written Text) on the Arch of Constantine (Human-made object) made by Rodolfo Lanciani between 1893 and 1901 \n
    - The reading of the Greek text present on the Derveni papyrus (Human-made object)"""@en.

  crmtex:TXP1_used_writing_system
    a owl:ObjectProperty ;
    skos:prefLabel "TXP1 used writing system"@en ;
    skos:notation "TXP1" ;
    rdfs:label "used writing system"@en ;
    rdfs:domain crmtex:TX2_Writing;
    rdfs:range crmtex:TX3_Writing_System;
    owl:inverseOf crmtex:TXP1i_writing_system_used_for;
    rdfs:subPropertyOf crm:P33_used_specific_technique;
    rdfs:comment """This property identifies the specific instance of Writing System employed during the writing event (TX2) that led to the creation of a 
    written text (Written Text).

    Examples:
    - The Roman stonecutter used writing system “Latin” (TX3) for the engraving (TX2) of the inscription on the Arch of Constantine (Written Text).
    - The Greek scribe used writing system “Greek” (TX3) to trace (TX2) in ink the letters that compose the text of the Papyrus of Derveni (Written Text).
    """@en .

  crmtex:TXP1i_writing_system_used_for
    a owl:ObjectProperty ;
    skos:prefLabel "TXP1i writing system used for"@en ;
    skos:notation "TXP1i" ;
    rdfs:label "writing system used for"@en ;
    rdfs:domain crmtex:TX3_Writing_System;
    rdfs:range crmtex:TX2_Writing;
    owl:inverseOf crmtex:TXP1_used_writing_system;
    rdfs:subPropertyOf crm:P33i_was_used_by;
    rdfs:comment """This property identifies the specific instance of Writing System employed during the writing event (TX2) that led to the creation of a 
    written text (Written Text).

    Examples:
    - The Roman stonecutter used writing system “Latin” (TX3) for the engraving (TX2) of the inscription on the Arch of Constantine (Written Text).
    - The Greek scribe used writing system “Greek” (TX3) to trace (TX2) in ink the letters that compose the text of the Papyrus of Derveni (Written Text).
    """@en .

  crmtex:TXP2_includes
    a owl:ObjectProperty ;
    skos:prefLabel "TXP2 includes"@en ;
    skos:notation "TXP2" ;
    rdfs:label "includes"@en ;
    rdfs:domain crmtex:TX4_Writing_Field;
    rdfs:range crmtex:TX1_Written_Text;
    owl:inverseOf crmtex:TXP2i_is_included_within;
    rdfs:subPropertyOf crm:P56_bears_feature;
    rdfs:comment """This property describes the relation existing between a Written Text and the Writing Field, specifically created 
    to accommodate the text, within which it is inscribed. This relation becomes quite relevant in the very frequent case where more 
    than a single text is found on different areas of a specific support.

    Examples:
    - The South framework (TX4) carved by the Roman stonecutter on top of the Arch includes the inscription on the South face of the Arch of Constantine (Written Text).
    """@en .

  crmtex:TXP2i_is_included_within
    a owl:ObjectProperty ;
    skos:prefLabel "TXP2i is included within"@en ;
    skos:notation "TXP2i" ;
    rdfs:label "is included within"@en ;
    rdfs:domain crmtex:TX1_Written_Text;
    rdfs:range crmtex:TX4_Writing_Field;
    owl:inverseOf crmtex:TXP2_includes;
    rdfs:subPropertyOf crm:P56i_is_found_on;
    rdfs:comment """This property describes the relation existing between a Written Text and the Writing Field, specifically created to accommodate 
    the text, within which it is inscribed. This relation becomes quite relevant in the very frequent case where more than a single 
    text is found on different areas of a specific support.

    Examples:
    - The South framework (TX4) carved by the Roman stonecutter on top of the Arch includes the inscription on the South face of the Arch of Constantine (Written Text).
    """@en .

  crmtex:TXP4_has_segment
    a owl:ObjectProperty ;
    skos:prefLabel "TXP4 has segment"@en ;
    skos:notation "TXP4" ;
    rdfs:label "has segment"@en ;
    rdfs:domain crmtex:TX1_Written_Text;
    rdfs:range crmtex:TX7_Written_Text_Segment;
    owl:inverseOf crmtex:TXP4i_is_segment_of;
    rdfs:subPropertyOf crm:P46_is_composed_of;
    rdfs:comment """This property is intended to correlate a text and the different parts of it which a scholar can identify, such as: letters, 
    words, lines, columns, pages, or any other scan that can be made by scholars because it is considered to have a particular 
    relevance for the investigation of the text itself.

    Examples:
    - The “INSTINCTV DIVINITATIS” text portion is segment of the inscription (Written Text) on the Arch of Constantine reported and commented by
     Rodolfo Lanciani in 1892 in his book Pagan and Christian Rome.
    """@en .

  crmtex:TXP4i_is_segment_of
    a owl:ObjectProperty ;
    skos:prefLabel "TXP4i is segment of"@en ;
    skos:notation "TXP4i" ;
    rdfs:label "is segment of"@en ;
    rdfs:domain crmtex:TX7_Written_Text_Segment;
    rdfs:range crmtex:TX1_Written_Text;
    owl:inverseOf crmtex:TXP4_has_segment;
    rdfs:subPropertyOf crm:P46i_forms_part_of;
    rdfs:comment """This property is intended to correlate a text and the different parts of it which a scholar can 
    identify, such as: letters, words, lines, columns, pages, or any other scan that can be made by scholars because 
    it is considered to have a particular relevance for the investigation of the text itself.

    Examples:
    - The “INSTINCTV DIVINITATIS” text portion is segment of the inscription (Written Text) on the Arch of Constantine reported and commented by 
    Rodolfo Lanciani in 1892 in his book Pagan and Christian Rome.
    """@en .

  crmtex:TXP5_wrote
    a owl:ObjectProperty ;
    skos:prefLabel "TXP5 wrote"@en ;
    skos:notation "TXP5" ;
    rdfs:label "wrote"@en ;
    rdfs:domain crmtex:TX2_Writing;
    rdfs:range crmtex:TX1_Written_Text;
    owl:inverseOf crmtex:TXP5i_was_written_by;
    rdfs:subPropertyOf crm:P108_has_produced;
    rdfs:comment """This property is used to describe in detail the close relationship between a text and the writing event that led to its production.

    Examples:
    - The activity (TX2) carried out by the Greek stonecutters wrote the Gortyn Law inscription (Written Text) on the wall of the Amphitheatre of Gortyn, Crete.
    """@en .

  crmtex:TXP5i_was_written_by
    a owl:ObjectProperty ;
    skos:prefLabel "TXP5i was written by"@en ;
    skos:notation "TXP5i" ;
    rdfs:label "was written by"@en ;
    rdfs:domain crmtex:TX1_Written_Text;
    rdfs:range crmtex:TX2_Writing;
    owl:inverseOf crmtex:TXP5_wrote;
    rdfs:subPropertyOf crm:P108i_was_produced_by;
    rdfs:comment """This property is used to describe in detail the close relationship between a text and the writing event that led to its production.

    Examples:
    - The activity (TX2) carried out by the Greek stonecutters wrote the Gortyn Law inscription (Written Text) on the wall of the Amphitheatre of Gortyn, Crete.
    """@en .

  crmtex:TXP6_encodes
    a owl:ObjectProperty ;
    skos:prefLabel "TXP6 encodes"@en ;
    skos:notation "TXP6" ;
    rdfs:label "encodes"@en ;
    rdfs:domain crmtex:TX3_Writing_System;
    rdfs:range crm:E56_Language;
    owl:inverseOf crmtex:TXP6i_is_encoding_of;
    rdfs:subPropertyOf crm:P2_has_type;
    rdfs:comment """This property is used to indicate the language encoded by the Writing System and used for writing, reading or rendering (i.e. transcribing) a Written Text.

    Examples:
    - The Latin alphabet (TX3), used to encode the identical inscriptions (Written Text) on the Arch of Constantine, encodes the Latin language 
    (E56) used to convey the message of the inscriptions.
    """@en .

  crmtex:TXP6i_is_encoding_of
    a owl:ObjectProperty ;
    skos:prefLabel "TXP6i is encoding of"@en ;
    skos:notation "TXP6i" ;
    rdfs:label "is encoding of"@en ;
    rdfs:domain crm:E56_Language;
    rdfs:range crmtex:TX3_Writing_System;
    owl:inverseOf crmtex:TXP6_encodes;
    rdfs:subPropertyOf crm:P2i_is_type_of;
    rdfs:comment """This property is used to indicate the language encoded by the Writing System and used for writing, reading or rendering 
    (i.e. transcribing) a Written Text.

    Examples:
    - The Latin alphabet (TX3), used to encode the identical inscriptions (Written Text) on the Arch of Constantine, encodes the Latin language 
    (E56) used to convey the message of the inscriptions.
    """@en .

  crmtex:TXP7_has_item
    a owl:ObjectProperty ;
    skos:prefLabel "TXP7 has item"@en ;
    skos:notation "TXP7" ;
    rdfs:label "has item"@en ;
    rdfs:domain crmtex:TX13_Script;
    rdfs:range crmtex:TX8_Grapheme;
    owl:inverseOf crmtex:TXP7i_is_item_of;
    rdfs:subPropertyOf crm:P67_refers_to;
    rdfs:comment """This property associates an instance of Script with an instance of Grapheme employed by this script. Different instances 
    of Script may have some graphemes in common.

    Examples:
    - The Latin script (TX13) has item the ideal capital letter “S”.
    """@en .

  crmtex:TXP7i_is_item_of
    a owl:ObjectProperty ;
    skos:prefLabel "TXP7i is item of"@en ;
    skos:notation "TXP7i" ;
    rdfs:label "is item of"@en ;
    rdfs:domain crmtex:TX8_Grapheme;
    rdfs:range crmtex:TX13_Script;
    owl:inverseOf crmtex:TXP7_has_item;
    rdfs:subPropertyOf crm:P67i_is_referred_to_by;
    rdfs:comment """This property associates an instance of Script with an instance of Grapheme employed by this script. Different instances of 
    Script may have some graphemes in common.

    Examples:
    - The Latin script (TX13) has item the ideal capital letter “S”.
    """@en .

  crmtex:TXP8_has_component
    a owl:ObjectProperty ;
    skos:prefLabel "TXP8 has component"@en ;
    skos:notation "TXP8" ;
    rdfs:label "has component"@en ;
    rdfs:domain crmtex:TX1_Written_Text;
    rdfs:range crmtex:TX9_Glyph;
    owl:inverseOf crmtex:TXP8i_is_component_of;
    rdfs:subPropertyOf crm:P46_is_composed_of;
    rdfs:comment """This property is used to state the (physical) belonging of a glyph to a given Written Text.

    Examples:
    - The inscription (Written Text) on the South face of the Arch of Constantine, has component the S-shaped glyph (TX9) engraved on the second 
    line, representing the letter (TX8) “S” of the Latin writing system (TX3).
    """@en .

  crmtex:TXP8i_is_component_of
    a owl:ObjectProperty ;
    skos:prefLabel "TXP8i is component of"@en ;
    skos:notation "TXP8i" ;
    rdfs:label "is component of"@en ;
    rdfs:domain crmtex:TX9_Glyph;
    rdfs:range crmtex:TX1_Written_Text;
    owl:inverseOf crmtex:TXP8_has_component;
    rdfs:subPropertyOf crm:P46i_forms_part_of;
    rdfs:comment """This property is used to state the (physical) belonging of a glyph to a given Written Text.

    Examples:
    - The inscription (Written Text) on the South face of the Arch of Constantine, has component the S-shaped glyph (TX9) engraved on the second
     line, representing the letter (TX8) “S” of the Latin writing system (TX3).
    """@en .

  crmtex:TXP9_is_encoded_using
    a owl:ObjectProperty ;
    skos:prefLabel "TXP9 is encoded using"@en ;
    skos:notation "TXP9" ;
    rdfs:label "is encoded using"@en ;
    rdfs:domain crmtex:TX1_Written_Text;
    rdfs:range crmtex:TX3_Writing_System;
    owl:inverseOf crmtex:TXP9i_was_used_to_encode;
    rdfs:comment """This property has the purpose of directly associating a Written Text with the Writing System used for encoding it. 
    It is a shortcut of the more fully articulated path from Written Text through TXP5i was written by, Writing, TXP1 used writing system to Writing System.

    Examples:
    - The Gortyn Law inscriptions (Written Text), engraved on the wall of the Amphitheatre of Gortyn (Crete), is encoded using the Greek alphabet (TX3).
    """@en .

  crmtex:TXP9i_was_used_to_encode
    a owl:ObjectProperty ;
    skos:prefLabel "TXP9i was used to encode"@en ;
    skos:notation "TXP9i" ;
    rdfs:label "was used to encode"@en ;
    rdfs:domain crmtex:TX3_Writing_System;
    rdfs:range crmtex:TX1_Written_Text;
    owl:inverseOf crmtex:TXP9_is_encoded_using;
    rdfs:comment """This property has the purpose of directly associating a Written Text with the Writing System used for encoding it. 
    It is a shortcut of the more fully articulated path from Written Text through TXP5i was written by, Writing, TXP1 used writing system to Writing System.

    Examples:
    - The Gortyn Law inscriptions (Written Text), engraved on the wall of the Amphitheatre of Gortyn (Crete), is encoded using the Greek alphabet (TX3).
    """@en .

  crmtex:TXP10_deciphered_text
    a owl:ObjectProperty ;
    skos:prefLabel "TXP10 deciphered text"@en ;
    skos:notation "TXP10" ;
    rdfs:label "deciphered text"@en ;
    rdfs:domain crmtex:TX5_Text_Recognition;
    rdfs:range crm:E24_Physical_Human-Made_Thing;
    owl:inverseOf crmtex:TXP10i_was_deciphered_by;
    rdfs:subPropertyOf crmsci:O8_observed;
    rdfs:comment """This property associates an instance of Text Recognition with an instance of Physical Human-Made Thing 
    carrying a glyph or a sequence of glyphs that was recognized in the respective activity of text recognition. Typically, 
    the associated instance of Physical Human-Made Thing is more specifically an instance of Written Text, however, a text may 
    also be recognized from a mechanical copy, a photograph, squeeze or other form of material copy of a written original, 
    which would not by itself constitute an instance of Written Text. In the latter case, the material copy should be associated 
    with the original written text using the property ‘P130 shows features’.
    If the text was actually recognized only from a digital representation, this property should not be used, rather the property 
    TXP13 deciphered via the representation should be used instead.

    Examples:
    - The autoptic investigation (TX5) carried out by Rodolfo Lanciani between 1893 and 1901, deciphered the South inscription
     (Written Text) on the Arch of Constantine.
    """@en .

  crmtex:TXP10i_was_deciphered_by
    a owl:ObjectProperty ;
    skos:prefLabel "TXP10i was deciphered by"@en ;
    skos:notation "TXP10i" ;
    rdfs:label "was deciphered by"@en ;
    rdfs:domain crm:E24_Physical_Human-Made_Thing;
    rdfs:range crmtex:TX5_Text_Recognition;
    owl:inverseOf crmtex:TXP10_deciphered_text;
    rdfs:subPropertyOf crmsci:O8i_was_observed_by;
    rdfs:comment """This property associates an instance of Text Recognition with an instance of Physical Human-Made Thing carrying 
    a glyph or a sequence of glyphs that was recognized in the respective activity of text recognition. Typically, 
    the associated instance of Physical Human-Made Thing is more specifically an instance of Written Text, however, 
    a text may also be recognized from a mechanical copy, a photograph, squeeze or other form of material copy of a 
    written original, which would not by itself constitute an instance of Written Text. In the latter case, the material 
    copy should be associated with the original written text using the property ‘P130 shows features’.
    If the text was actually recognized only from a digital representation, this property should not be used, rather the 
    property TXP13 deciphered via the representation should be used instead.

    Examples:
    - The autoptic investigation (TX5) carried out by Rodolfo Lanciani between 1893 and 1901, deciphered the South inscription
     (Written Text) on the Arch of Constantine.
    """@en .

  crmtex:TXP11_transcribed
    a owl:ObjectProperty ;
    skos:prefLabel "TXP11 transcribed"@en ;
    skos:notation "TXP11" ;
    rdfs:label "transcribed"@en ;
    rdfs:domain crmtex:TX6_Transliteration;
    rdfs:range crmtex:TX12_Grapheme_Sequence;
    owl:inverseOf crmtex:TXP11i_was_transcribed_by;
    rdfs:subPropertyOf crm:P16_used_specific_object;
    rdfs:comment """This property describes the relation between an activity of Transliteration and the identified sequence of graphemes (TX12) 
    represented in an instance of Written Text.

    Examples:
    - The transcription (TX6) of the S-shaped feature engraved on the second line of the South inscription of the Arch of Constantine transcribed 
    the prototypical letter “S” (TX8) of the Latin writing system (TX3).
    """@en .

  crmtex:TXP11i_was_transcribed_by
    a owl:ObjectProperty ;
    skos:prefLabel "TXP11i was transcribed by"@en ;
    skos:notation "TXP11i" ;
    rdfs:label "was transcribed by"@en ;
    rdfs:domain crmtex:TX12_Grapheme_Sequence;
    rdfs:range crmtex:TX6_Transliteration;
    owl:inverseOf crmtex:TXP11_transcribed;
    rdfs:subPropertyOf crm:P16i_was_used_for;
    rdfs:comment """This property describes the relation between an activity of Transliteration and the identified sequence of graphemes (TX12) represented 
    in an instance of Written Text.

    Examples:
    - The transcription (TX6) of the S-shaped feature engraved on the second line of the South inscription of the Arch of Constantine transcribed the 
    prototypical letter “S” (TX8) of the Latin writing system (TX3).
    """@en .

  crmtex:TXP12_has_style
    a owl:ObjectProperty ;
    skos:prefLabel "TXP12 has style"@en ;
    skos:notation "TXP12" ;
    rdfs:label "has style"@en ;
    rdfs:domain crmtex:TX1_Written_Text;
    rdfs:range crmtex:TX10_Style;
    owl:inverseOf crmtex:TXP12i_is_style_of;
    rdfs:subPropertyOf crm:P33_used_specific_technique;
    rdfs:comment """This property describes information about the style used for the realization of the written text (Written Text). The property TXP12.1 
    has type allows the nature of the style to be specified, for example to record the direction, orientation or the linear system of the text.

    Examples:
    - The Latin text in the Carolingian Gospel Book identified as “British Library, Add MS 11848, has style “Carolingian minuscule”
    - The inscription (Written Text) on the Arch of Constantine has style ductus (TX10) has type dextroverse (E55)

    Properties:
    - TXP12.1 has type
    """@en .

  crmtex:TXP12i_is_style_of
    a owl:ObjectProperty ;
    skos:prefLabel "TXP12i is style of"@en ;
    skos:notation "TXP12i" ;
    rdfs:label "is style of"@en ;
    rdfs:domain crmtex:TX10_Style;
    rdfs:range crmtex:TX1_Written_Text;
    owl:inverseOf crmtex:TXP12_has_style;
    rdfs:subPropertyOf crm:P33i_was_used_by;
    rdfs:comment """This property describes information about the style used for the realization of the written 
    text (Written Text). The property TXP12.1 has type allows the nature of the style to be specified, for example to record 
    the direction, orientation or the linear system of the text.

    Examples:
    - The Latin text in the Carolingian Gospel Book identified as “British Library, Add MS 11848, has style “Carolingian minuscule”
    - The inscription (Written Text) on the Arch of Constantine has style ductus (TX10) has type dextroverse (E55)
    """@en .

  crmtex:TXP13_deciphered_via_the_representation
    a owl:ObjectProperty ;
    skos:prefLabel "TXP13 deciphered via the representation"@en ;
    skos:notation "TXP13" ;
    rdfs:label "deciphered via the representation"@en ;
    rdfs:domain crmtex:TX5_Text_Recognition;
    rdfs:range crm:E36_Visual_Item;
    owl:inverseOf crmtex:TXP13i_was_representation_used_for_deciphering;
    rdfs:subPropertyOf crm:P16_used_specific_object;
    rdfs:comment """This property associates an instance of Text Recognition with an instance of Visual Item, capturing the optical 
    impression of an instance of Written Text by some mechanical method, that was used for recognizing the text without access to 
    the original text and without an explicitly documented material copy or electronic display device that was used for the process.
    If the text was actually recognized from an autoptic recognition or from a material reproduction, this property may not be used but 
    the property “TXP10 deciphered text (was deciphered by)” should be used instead.
    This property should also not be used, if the recognition of the text was actually carried out from the original text or a material 
    copy of it together with an auxiliary instance of Visual Item. In this case, the use of the auxiliary material should be documented 
    with the more general property P16 used specific object.

    Examples:
    - The recognition of text in the Antikythera mechanism (TX5) deciphered via the representation produced using BTI imaging (E36).
    """@en .

  crmtex:TXP13i_was_representation_used_for_deciphering
    a owl:ObjectProperty ;
    skos:prefLabel "TXP13i was representation used for deciphering"@en ;
    skos:notation "TXP13i" ;
    rdfs:label "was representation used for deciphering"@en ;
    rdfs:domain crm:E36_Visual_Item;
    rdfs:range crmtex:TX5_Text_Recognition;
    owl:inverseOf crmtex:TXP13_deciphered_via_the_representation;
    rdfs:subPropertyOf crm:P16i_was_used_for;
    rdfs:comment """This property associates an instance of Text Recognition with an instance of Visual Item, capturing the optical 
    impression of an instance of Written Text by some mechanical method, that was used for recognizing the text without access to the 
    original text and without an explicitly documented material copy or electronic display device that was used for the process.
    If the text was actually recognized from an autoptic recognition or from a material reproduction, this property may not be used but 
    the property “TXP10 deciphered text (was deciphered by)” should be used instead.
    This property should also not be used, if the recognition of the text was actually carried out from the original text or a material 
    copy of it together with an auxiliary instance of Visual Item. In this case, the use of the auxiliary material should be documented 
    with the more general property P16 used specific object.

    Examples:
    - The recognition of text in the Antikythera mechanism (TX5) deciphered via the representation produced using BTI imaging (E36).
    """@en .

  crmtex:TXP14_used_copy_or_representation_of
    a owl:ObjectProperty ;
    skos:prefLabel "TXP14 used copy or representation of"@en ;
    skos:notation "TXP14" ;
    rdfs:label "used copy or representation of"@en ;
    rdfs:domain crmtex:TX5_Text_Recognition;
    rdfs:range crmtex:TX1_Written_Text;
    owl:inverseOf crmtex:TXP14i_was_deciphered_via_copy_or_representation;
    rdfs:subPropertyOf crm:P16_used_specific_object;
    rdfs:comment """This property associates an instance of Text Recognition, carried out only via copies or representations 
    of a text, with the original instance of Written Text that was represented on the used copies or digital surrogates.
    This property is to be used only for non-autoptic recognition. If this particular recognition of the text was actually carried 
    out from the original text, the property TXP10 deciphered text should be used for associating the instance of Text Recognition 
    with the original instance of Written Text.
    If some form of material copy of the written text was used for the text recognition, then this material copy should be associated 
    with the original written text using the property ‘P130 shows features of’.

    Examples:
    - The non-autoptic recognition of the inscription text on the Arch of Constantine (TX5) used a copy or representation of the written text 
    (Written Text) on the Arch of Constantine [performed using a photo of the arch].
    """@en .

  crmtex:TXP14i_was_deciphered_via_copy_or_representation
    a owl:ObjectProperty ;
    skos:prefLabel "TXP14i was deciphered via copy or representation"@en ;
    skos:notation "TXP14i" ;
    rdfs:label "was deciphered via copy or representation"@en ;
    rdfs:domain crmtex:TX1_Written_Text;
    rdfs:range crmtex:TX5_Text_Recognition;
    owl:inverseOf crmtex:TXP14_used_copy_or_representation_of;
    rdfs:subPropertyOf crm:P16i_was_used_for;
    rdfs:comment """This property associates an instance of Text Recognition, carried out only via copies or representations 
    of a text, with the original instance of Written Text that was represented on the used copies or digital surrogates.
    This property is to be used only for non-autoptic recognition. If this particular recognition of the text was actually carried 
    out from the original text, the property TXP10 deciphered text should be used for associating the instance of Text Recognition 
    with the original instance of Written Text.
    If some form of material copy of the written text was used for the text recognition, then this material copy should be associated 
    with the original written text using the property ‘P130 shows features of’.

    Examples:
    - The non-autoptic recognition of the inscription text on the Arch of Constantine (TX5) used a copy or representation of the written 
    text (Written Text) on the Arch of Constantine [performed using a photo of the arch].
    """@en .

  crmtex:TXP15_recorded_correspondence
    a owl:ObjectProperty ;
    skos:prefLabel "TXP15 recorded correspondence"@en ;
    skos:notation "TXP15" ;
    rdfs:label "recorded correspondence"@en ;
    rdfs:domain crmtex:TX5_Text_Recognition;
    rdfs:range crmtex:TX12_Grapheme_Sequence;
    owl:inverseOf crmtex:TXP15i_was_recorded_by;
    rdfs:subPropertyOf crm:P94_has_created;
    rdfs:comment """This property associates an instance of Text Recognition with an instance of Grapheme Sequence 
    that was created by this activity of text recognition for recording and representing as faithfully as possible 
    the exact value of each sign on the physical material of the recognized instance of Written Text.

    Examples:
    - The autoptic investigation carried out by Rodolfo Lanciani (TX5) recorded correspondence the grapheme sequence ‘INSTINCTV DIVINITATIS’ 
    on the Arch of Constantine (TX12) .
    """@en .

  crmtex:TXP15i_was_recorded_by
    a owl:ObjectProperty ;
    skos:prefLabel "TXP15i was recorded by"@en ;
    skos:notation "TXP15i" ;
    rdfs:label "was recorded by"@en ;
    rdfs:domain crmtex:TX12_Grapheme_Sequence;
    rdfs:range crmtex:TX5_Text_Recognition;
    owl:inverseOf crmtex:TXP15_recorded_correspondence;
    rdfs:subPropertyOf crm:P94i_was_created_by;
    rdfs:comment """This property associates an instance of Text Recognition with an instance of Grapheme Sequence 
    that was created by this activity of text recognition for recording and representing as faithfully as possible 
    the exact value of each sign on the physical material of the recognized instance of Written Text.

    Examples:
    - The autoptic investigation carried out by Rodolfo Lanciani (TX5) recorded correspondence the grapheme sequence ‘INSTINCTV DIVINITATIS’ 
    on the Arch of Constantine (TX12) .
    """@en .

  crmtex:TXP16_employs_script
    a owl:ObjectProperty ;
    skos:prefLabel "TXP16 employs script"@en ;
    skos:notation "TXP16" ;
    rdfs:label "employs script"@en ;
    rdfs:domain crmtex:TX3_Writing_System;
    rdfs:range crmtex:TX13_Script;
    owl:inverseOf crmtex:TXP16i_is_employed_by;
    rdfs:subPropertyOf crm:P148_has_component;
    rdfs:comment """This property associates an instance of Writing System with one of the instances of the script (TX13) it employs.

    Examples:
    - The Latin writing system used in the inscription of the Arch of Constantine (TX3) employs script the Latin script (TX13).
    - The Oscan writing system used in the inscription of the Tabula Bantina (TX3) employs script the Latin script (TX13).
    - The Oscan writing system (TX3) used in the inscription of the Arch of Constantine employs script the Greek script (TX13).
    """@en .

  crmtex:TXP16i_is_employed_by
    a owl:ObjectProperty ;
    skos:prefLabel "TXP16i is employed by"@en ;
    skos:notation "TXP16i" ;
    rdfs:label "is employed by"@en ;
    rdfs:domain crmtex:TX13_Script;
    rdfs:range crmtex:TX3_Writing_System;
    owl:inverseOf crmtex:TXP16_employs_script;
    rdfs:subPropertyOf crm:P148i_is_component_of;
    rdfs:comment """This property associates an instance of Writing System with one of the instances of the script (TX13) it employs.

    Examples:
    - The Latin writing system used in the inscription of the Arch of Constantine (TX3) employs script the Latin script (TX13).
    - The Oscan writing system used in the inscription of the Tabula Bantina (TX3) employs script the Latin script (TX13).
    - The Oscan writing system (TX3) used in the inscription of the Arch of Constantine employs script the Greek script (TX13).
    """@en .

  crmtex:TXP17_has_part
    a owl:ObjectProperty ;
    skos:prefLabel "TXP17 has part"@en ;
    skos:notation "TXP17" ;
    rdfs:label "has part"@en ;
    rdfs:domain crmtex:TX12_Grapheme_Sequence;
    rdfs:range crmtex:TX12_Grapheme_Sequence;
    owl:inverseOf crmtex:TXP17i_forms_part_of;
    rdfs:subPropertyOf crm:P106_is_composed_of;
    rdfs:comment """This property associates an instance of Grapheme Sequence with another instance of Grapheme 
    Sequence appearing at a particular position of the sequence. The property can be also used by an instance of 
    Grapheme Occurrence (subclass of Grapheme Sequence) for denoting that a grapheme occurrence has part another 
    grapheme occurrence. Note that a grapheme occurrence may be a symbolic composite containing another grapheme 
    occurrence, such as the minute character “e” on top of the character “u” in former German writing systems 
    denoting the symbol for “ü”.

    Examples:
    - The “DIVINITATIS” grapheme sequence (TX12), corresponding to the glyph sequence of the inscription (Written Text) on the Arch of 
    Constantine, has part the “AT” grapheme sequence (TX12) [which appears to be damaged].
    """@en .

  crmtex:TXP17i_forms_part_of
    a owl:ObjectProperty ;
    skos:prefLabel "TXP17i forms part of"@en ;
    skos:notation "TXP17i" ;
    rdfs:label "forms part of"@en ;
    rdfs:domain crmtex:TX12_Grapheme_Sequence;
    rdfs:range crmtex:TX12_Grapheme_Sequence;
    owl:inverseOf crmtex:TXP17_has_part;
    rdfs:subPropertyOf crm:P106i_forms_part_of;
    rdfs:comment """This property associates an instance of Grapheme Sequence with another instance of Grapheme 
    Sequence appearing at a particular position of the sequence. The property can be also used by an instance of 
    Grapheme Occurrence (subclass of Grapheme Sequence) for denoting that a grapheme occurrence has part another 
    grapheme occurrence. Note that a grapheme occurrence may be a symbolic composite containing another grapheme 
    occurrence, such as the minute character “e” on top of the character “u” in former German writing systems 
    denoting the symbol for “ü”.

    Examples:
    - The “DIVINITATIS” grapheme sequence (TX12), corresponding to the glyph sequence of the inscription (Written Text) on the Arch of 
    Constantine, has part the “AT” grapheme sequence (TX12) [which appears to be damaged].
    """@en .

  crmtex:TXP18_read
    a owl:ObjectProperty ;
    skos:prefLabel "TXP18 read"@en ;
    skos:notation "TXP18" ;
    rdfs:label "read"@en ;
    rdfs:domain crmtex:TX14_Reading;
    rdfs:range crmtex:TX1_Written_Text;
    owl:inverseOf crmtex:TXP18i_was_read_by;
    rdfs:subPropertyOf crm:P16_used_specific_object;
    rdfs:comment """This property associates an instance of Reading with an instance of Written Text whose 
    linguistic meaning was interpreted/understood through the reading process. It is a shortcut of the fully 
    developed path from Reading through P9 consists of, Text Recognition, TXP10 deciphered text, to Written Text.

    Examples:
    - Reading the Greek text present on the Derveni papyrus (TX14) read the papyrus (Written Text) [interpreted the linguistic meaning that was carried by it]
    """@en .

  crmtex:TXP18i_was_read_by
    a owl:ObjectProperty ;
    skos:prefLabel "TXP18i was read by"@en ;
    skos:notation "TXP18i" ;
    rdfs:label "was read by"@en ;
    rdfs:domain crmtex:TX1_Written_Text;
    rdfs:range crmtex:TX14_Reading;
    owl:inverseOf crmtex:TXP18_read;
    rdfs:subPropertyOf crm:P16i_was_used_for;
    rdfs:comment """This property associates an instance of Reading with an instance of Written Text whose 
    linguistic meaning was interpreted/understood through the reading process. It is a shortcut of the fully 
    developed path from Reading through P9 consists of, Text Recognition, TXP10 deciphered text, to Written Text.

    Examples:
    - Reading the Greek text present on the Derveni papyrus (TX14) read the papyrus (Written Text) [interpreted the linguistic meaning that was carried by it]
    """@en .
}