@prefix rs: <http://www.researchspace.org/ontology/> .
@prefix User: <http://www.researchspace.org/resource/user/> .
@prefix Help: <http://help.researchspace.org/resource/> .
@prefix Platform: <http://www.researchspace.org/resource/system/> .
@prefix owl: <http://www.w3.org/2002/07/owl#> .
@prefix xsd: <http://www.w3.org/2001/XMLSchema#> .
@prefix skos: <http://www.w3.org/2004/02/skos/core#> .
@prefix rdfs: <http://www.w3.org/2000/01/rdf-schema#> .
@prefix crmdig: <http://www.cidoc-crm.org/extensions/crmdig/> .
@prefix rsp: <http://www.researchspace.org/resource/> .
@prefix rshelp: <http://researchspace.org/help/> .
@prefix crmsci: <http://www.cidoc-crm.org/extensions/crmsci/> .
@prefix crmgeo: <http://www.cidoc-crm.org/extensions/crmgeo/> .
@prefix sp: <http://spinrdf.org/sp#> .
@prefix prov: <http://www.w3.org/ns/prov#> .
@prefix crminfluence: <http://www.cidoc-crm.org/extensions/influence/> .
@prefix crm: <http://www.cidoc-crm.org/cidoc-crm/> .
@prefix crminf: <http://www.cidoc-crm.org/extensions/crminf/> .
@prefix Admin: <http://www.researchspace.org/resource/admin/> .
@prefix bds: <http://www.bigdata.com/rdf/search#> .
@prefix rdf: <http://www.w3.org/1999/02/22-rdf-syntax-ns#> .
@prefix crmba: <http://www.cidoc-crm.org/extensions/crmba/> .
@prefix ontodia: <http://ontodia.org/schema/v1#> .
@prefix crmarchaeo: <http://www.cidoc-crm.org/extensions/crmarchaeo/> .
@prefix forms: <http://www.researchspace.org/resource/system/forms/> .
@prefix lrmoo: <http://iflastandards.info/ns/lrm/lrmoo/> .
@prefix crmtex: <http://www.cidoc-crm.org/extensions/crmtex/> .

crmgeo:context {

  <http://www.cidoc-crm.org/extensions/crmgeo/> a owl:Ontology;
    rdfs:comment """CRMgeo is an ontology intended to be used as a schema for integrating geoinformation using the conceptualizations,
    formal definitions, encoding standards and topological relations defined by the Open Geospatial Consortium (OGC). 
    In order to do this it links the CIDOC CRM to the OGC standard of GeoSPARQL."""@en;
    owl:versionInfo "1.2"@en;
    rdfs:label "CRMgeo v1.2"@en .

  crmgeo:SP1_Phenomenal_Spacetime_Volume 
    a owl:Class ;
    skos:prefLabel "SP1 Phenomenal Spacetime Volume"@en ;
    skos:notation "SP1" ;
    rdfs:label "Phenomenal Spacetime Volume"@en ;
    rdfs:subClassOf crm:E92_Spacetime_Volume;
    rdfs:comment """This class comprises the 4 dimensional point sets (volumes) (S) which material phenomena (I) occupy in Space-Time (S). 
    An instance of Space Time Volume represents the true (I) extent of an instance of E4 Period in spacetime or the true (I) 
    extent of the trajectory of an instance of Physical Thing during the course of its existence, from production to destruction. 
    A fuzziness of the extent lies in the very nature of the phenomenon, and not in the shortcomings of observation (U). 
    The degree of fuzziness with respect to the scale of the phenomenon may vary widely, but the extent is never exact in a mathematical sense. 
    According to modern physics, points in space-time are absolute with respect to the physical phenomena happening at them, 
    regardless the so-called Galilean relativity of spatial or temporal reference systems in terms of which an observer may describe them. 
    Following the theory, points relative to different spatial or temporal reference systems can be related if common points of phenomena 
    in space-time are known in different systems. Instances of Phenomenal Space-Time Volume are sets of such absolute space-time points of phenomena (I).
    The (Einstein) relativity of spatial and temporal distances is of no concern for the scales of things in the cultural-historical discourse, 
    but does not alter the above principles. The temporal projection of an instance of Phenomenal Space-Time Volume defines an Time-Span while its 
    spatial projection defines an Phenomenal Place. The true location of an instance of Physical Thing during some time-span can be regarded as the 
    spatial projection of the restriction of its trajectory to the respective time-span.
    """@en ;
    skos:example """- The Space Time Volume of the Event of Ceasars murdering \n
    - The Space Time Volume where and when the carbon 14 dating of the "Schoeninger Speer II" in 1996 took place \n
    - The spatio-temporal trajectory of the H.M.S. Victory from its building to its actual location \n
    - The Space Time Volume of the temple in Abu Simbel before its removal"""@en.

  crmgeo:SP2_Phenomenal_Place 
    a owl:Class ;
    skos:prefLabel "SP2 Phenomenal Place"@en ;
    skos:notation "SP2" ;
    rdfs:label "Phenomenal Place"@en ;
    rdfs:subClassOf crm:E53_Place;
    rdfs:comment """This class comprises instances of Place (S) whose extent (U) and position is defined by the spatial projection 
    of the spatiotemporal extent of a real world phenomenon that can be observed or measured. The spatial projection depends on the instance of 
    Reference Space onto which the extent of the phenomenon is projected. In general, there are no limitations to the 
    number of Reference Spaces one could regard, but only few choices are relevant for the cultural-historical discourse. 
    Typical for the archaeological discourse is to choose a reference space with respect to which the remains of some events 
    would stay at the same place, for instance, relative to the bedrock of a continental plate. On the other side, for the 
    citizenship of babies born in aeroplanes, the space in which the boundaries of the overflown state are defined may be relevant (I). 
    Instances of Phenomenal Place exist as long as the respective reference space is defined. Note that we can talk in particular about 
    what was at a place in a country before a city was built there, i.e., before the time the event occurred by which the place is defined, 
    but we cannot talk about the place of earth before it came into existence due to lack of a reasonable reference space (E).
    """@en ;
    skos:example """- The place where the murder of Ceasar happened \n
    - Place on H.M.S. Victory at which Nelson died \n
    - The Place of the Varus Battle \n
    - The volume in space of my vine glass \n
    - The place the H.M.S Victory occupied over the seafloor when Nelson died \n
    - The space enclosed by this room \n
    - The space in borehole Nr. 405"""@en.

  crmgeo:SP3_Reference_Space 
    a owl:Class ;
    skos:prefLabel "SP3 Reference Space"@en ;
    skos:notation "SP3" ;
    rdfs:label "Reference Space"@en ;
    rdfs:subClassOf crm:E1_CRM_Entity;
    rdfs:comment """This class comprises the (typically Euclidian) Space (S) that is at rest (I) in relation to an instance of Physical Thing 
    and extends (U) infinitely beyond it. It is the space in which we typically expect things to stay in place if no particular 
    natural or human distortion processes occur. This definition requires that at least essential parts of the respective physical 
    thing have a stability of form. The degree of this stability (e.g., elastic deformation of a ship on sea, landslides, geological 
    deformations) limits the precision to which an instance of Reference Space is defined. It is possible to construct types of (non Euclidian) 
    reference spaces which adapt to elastic deformations or have other geometric and dynamic properties to adapt to changes of form of the reference object, 
    but they are of rare utility in the cultural-historical discourse. 
    An instance of Reference Space begins to exist with the largest thing that is at rest in it and ceases to exist with its Destruction. 
    If other things are at rest in the same space and their time-span of existence falls within the one of the reference object, they share the same reference space (I). 
    It has therefore the same temporal extent (time-span of existence) as the whole of the Physical Things it is at rest with (E).
    """@en ;
    skos:example """- The Space inside and around H.M.S. Victory while it is moving through the Atlantic Ocean \n
    - The Space inside and around the Eurasian Continental Plate \n
    - The Space inside and around the Earth \n
    - The Space inside and around the Solar system"""@en.

  crmgeo:SP4_Spatial_Coordinate_Reference_System 
    a owl:Class ;
    skos:prefLabel "SP4 Spatial Coordinate Reference System"@en ;
    skos:notation "SP4" ;
    rdfs:label "Spatial Coordinate Reference System"@en ;
    rdfs:subClassOf crm:E29_Design_or_Procedure ;
    rdfs:comment """This class compromises systems that are used to describe locations in a Reference Space (S). 
    An instance of Spatial Coordinate Reference System is composed of two parts: The first is a Coordinate System which 
    is a set of coordinate axes with specified units of measurement and axis directions. The second part is a set of 
    reference features at rest in the Reference Space it describes in the real world that relate the Coordinate System to 
    real world locations (U) and fix it with respect to the reference object of its Reference Space .
    In surveying and geodesy, instance of Spatial Coordinate Reference System are called a datum. In the case of spatial 
    coordinate reference systems for the earth the datum consists of the reference points and an ellipsoid that approximates 
    the shape of the earth. National systems often use ellipsoids that approximate their territory best and shift them in an 
    appropriate position relative to the earth while WGS84 is an ellipsoid for the whole earth and used in GPS receivers. In 
    engineering a datum is a reference feature of an object used to create a reference system for measurement.The set of reference 
    features in the real world are subset of Physical Feature that are within the described reference space at rest and 
    pertain to the Physical Thing the reference space is at rest with.
    Spatial Coordinate Reference Systems have a validity for a certain spatial extent of the Reference Space and in addition a temporal validity. 
    The combination of coordinate reference system and datum provides a unique identity (I). Spatial Coordinate Reference Systems may 
    be defined for the earth, moving objects like planes or ships, linear features like boreholes or local systems. If there is a 
    standardised identifier system available, such as EPSG codes, it should be used.
    """@en ;
    skos:example """- Longitude-Latitude(ellipsoidal Coordinate System) in WGS84 (Datum) \n
    - EPSG 3241 \n
    - the coordinate system to describe locations on H.M.S. Victory taking the deck foundation of the middle mast as origin, the mast as z axis, the line at right angle to the bow line as x axis and a right angle to both as y axis  \n
    - The printed lines of the millimeter paper on which an archaeological feature is drawn"""@en.

  crmgeo:SP6_Declarative_Place 
    a owl:Class ;
    skos:prefLabel "SP6 Declarative Place"@en ;
    skos:notation "SP6" ;
    rdfs:label "Declarative Place"@en ;
    rdfs:subClassOf crm:E53_Place;
    rdfs:comment """This class comprises instances of Place (S) whose extent (U) and position is defined by an Space Primitive (S). 
    There is one implicit or explicit Reference Space in which the Geometric Place Expression describes the intended place. 
    Even though Geometric Place Expressions have an unlimited precision, measurement devices and the precision of the position 
    of reference features relating the Spatial Coordinate Reference System to a Reference Space impose limitations to the determination of a 
    Declarative Place in the real world (U).
    Several Geometric Place Expressions may denote the same Declarative Place if their precision falls within the same range (I).
    Instances of Declarative Places may be used to approximate instances of Places or parts of them. They may as well be used to define the 
    location and spatial extent of property rights or national borders.
    """@en ;
    skos:example """- the place defined by <gml:Point gml:id="p21" srsName="http://www.opengis.net/def/crs/EPSG/0/4326"> <gml:coordinates>45.67, 88.56</gml:coordinates> </gml:Point> \n
    - the place defined by a line approximating the Danube river \n
    - The place of the Orinoco river defined in the map of Diego Ribeiro \n
    - the place defined through a polygon that represents the boundaries of the UK in the year 2003"""@en.

  crmgeo:SP7_Declarative_Spacetime_Volume 
    a owl:Class ;
    skos:prefLabel "SP7 Declarative Spacetime Volume"@en ;
    skos:notation "SP7" ;
    rdfs:label "Declarative Spacetime Volume"@en ;
    rdfs:subClassOf crm:E92_Spacetime_Volume;
    rdfs:comment """This class comprises instances of Spacetime Volumes (S) whose temporal and spatial extent (U) and position is defined by a 
    Spacetime Volume Expression. There is one implicit or explicit Reference Space in which the Spacetime Volume Expression describes 
    the intended Spacetime Volume. As we restrict the model to Galilean physics and explicitly exclude systems with velocities close to 
    the speed of light we do not model a “Reference Time” as it would be necessary for relativistic physics. This implies that there is 
    only one Reference Time. 
    Even though Spacetime Volume Expressions have an unlimited precision, measurement devices and the precision of the position 
    of reference features relating the Spatial Coordinate Reference System to a Reference Space impose limitations to the determination 
    of the spatial part of a Declarative Spacetime Volume in the real world (U).
    The same limitation to precision is true for the temporal part of a Declarative Spacetime Volume due to precision of time measurement 
    devices and of the determination of the reference event of a Temporal Reference System. 
    Several Spacetime Volume Expressions may denote the same Declarative Spacetime Volume if their precision falls within the same range (I).
    Instances of Declarative Spacetime Volumes may be used to approximate instances of Spacetime Volumes or parts of them. They may as 
    well be used to define the spatial and temporal extent of property rights or national borders.
    """@en ;
    skos:example """- the spacetime volume defined by a polygon approximating the Danube river flood in Austria between 6(th) and 9(th) of August 2002 \n
    - the spacetime volume of the Orinoco river in 1529 defined in the map of Diego Ribeiro in 1529 \n
    - the spacetime volume representing the boundaries of the UK from 1900-1950"""@en.

  crmgeo:SP10_DeclarativeTime-Span 
    a owl:Class ;
    skos:prefLabel "SP10 Declarative Time-Span"@en ;
    skos:notation "SP10" ;
    rdfs:label "Declarative Time-Span"@en ;
    rdfs:subClassOf crm:E52_Time-Span;
    rdfs:comment """This class comprises instances of Time-Spans that represent the Time Span defined by a Time Expression. 
    Thus they derive their identity through an expression defining an extent in time. Even though Declarative 
    Time Spans have an unlimited precision, measurement devices and the possible precision within the Temporal Reference System impose 
    limitations to the determination of a Declarative Time Span. The accuracy of a Declarative Time Spans depends upon the documentation and measurement method. 
    Declarative Time Spans may be used to approximate actual (phenomenal) Time-Spans of temporal entities.
    """@en ;
    skos:example """- Extent in time defined by the expression “1961” \n
    - Extent in time defined by the expression “From 12-17-1993 to 12-8-1996” \n
    - Extent in time defined by the expression “14h30 – 16h22 4th July 1945”"""@en.

  crmgeo:SP11_Temporal_Reference_System 
    a owl:Class ;
    skos:prefLabel "SP11 Temporal Reference System"@en ;
    skos:notation "SP11" ;
    rdfs:label "Temporal Reference System"@en ;
    rdfs:subClassOf crm:E29_Design_or_Procedure ;
    rdfs:comment """This class compromises systems(S) that are used to describe positions and extents in a Reference Time. If relativistic effects are negligible 
    in the wider spacetime area of interest and the speeds of associated things, then there is only one unique global reference time. The typical way to measure 
    time is to count the cycles of a periodic process for which we have a hypothesis of constant frequency, such as oscillations of a crystal, molecular arrangement, 
    rotation of earth around itself or around the sun. The origin for a Temporal Reference System is fixed on a reference event. As long as the number of cycles 
    passed from that reference event until now are known, the temporal reference system exists (E) and expressions in this Reference System can be interpreted 
    with respect to the Reference Time. 
    A temporal reference system represents time as a continuous linear interpolation over the infinit series of cycles extended from the reference event to he 
    past and the future, regardless of the temporal position of the mathematical point zero of an instance of Time Expression, such for instance the gregorian 
    calender begins with the event an arbitrary positiong the point zero as beeing the date of the „Birth of Christ“. The actual date of birth of christ is regarded 
    to be unknown and therefor is not the reference event. 
    The identity of a Temporal Reference System is defined through the type of periodic process it is based on, the reference event and through the distance of the 
    reference event to the position of the mathematical point zero (I).
    A value in the Reference Time is a temporal position measured relative to a temporal reference system. ISO 8601 specifies the use of the Gregorian Calendar and 
    24 hour local or Coordinated Universal Time (UTC) for information interchange. 
    In ISO 19108 three common types of temporal reference systems are explicitly stated: calendars (used with clocks for greater resolution), temporal coordinate systems, 
    and ordinal temporal reference systems. 
    Calendars and clocks are both based on interval scales. A calendar is a discrete temporal reference system that provides a basis for defining temporal position to a 
    resolution of one day. A clock provides a basis for defining temporal position within a day. A clock must be used with a calendar in order to provide a complete 
    description of a temporal position within a specific day. Every calendar provides a set of rules for composing a calendar date from a set of elements such as year, 
    month, and day. In every calendar, years are numbered relative to the date of a reference event that defines a calendar era [ISO 19108].
    Specifying temporal position in terms of calendar date and time of day complicates the computation of distances between points and the functional description of 
    temporal operations. A temporal coordinate system may be used to support applications of this kind. [ISO 19108].
    Ordinal temporal reference systems as specified in ISO 19108 are no instances of Temporal Reference Systems as they do not define cycles of a periodic process but 
    define a system of time intervals based on reverence periods related to certain natural or cultural phenomena.
    """@en ;
    skos:example """- Gregorian Calendar \n
    - Coordinated Universal Time (UTC) \n
    - Julian date \n
    - Greenwich time \n
    - ISO 8601"""@en.

  crmgeo:SP13_Phenomenal_Time-Span 
    a owl:Class ;
    skos:prefLabel "SP13 Phenomenal Time-Span"@en ;
    skos:notation "SP13" ;
    rdfs:label "Phenomenal Time-Span"@en ;
    rdfs:subClassOf crm:E52_Time-Span;
    rdfs:comment """This class comprises instances of Time-Spans whose extent (U) and position is defined by the temporal projection of the spatiotemporal 
    extent that can be observed or measured. Thus they derive their identity through the extent in time of a real world phenomenon (I).
    """@en ;
    skos:example """- Duration of the phenomenal temporal extent of the Trafalgar battle \n
    - The real duration of the Ming Dynasty \n
    - The real extent of the lifetime of Ceasar starting with his birth and ending with his death"""@en.

  crm:E4_Period rdfs:subClassOf <http://www.opengis.net/ont/geosparql#Feature> .
  crm:E18_Physical_Thing rdfs:subClassOf <http://www.opengis.net/ont/geosparql#Feature> .
  <http://www.opengis.net/ont/geosparql#Geometry> rdfs:subClassOf crmgeo:SP6_Declarative_Place, crmgeo:SP7_Declarative_Spacetime_Volume .

  crmgeo:Q6_is_at_rest_in_relation_to 
    a owl:ObjectProperty ;
    skos:prefLabel "Q6 is at rest in relation to"@en ;
    skos:notation "Q6" ;
    rdfs:label "is at rest in relation to"@en ;
    rdfs:domain crmgeo:SP3_Reference_Space;
    rdfs:range crm:E18_Physical_Thing;
    owl:inverseOf crmgeo:Q6i_rests_in_relation_to;
    rdfs:comment """This property associates an instance of Reference Space with the instance of Physical Thing that 
    is at rest in it. For all instances of Physical Thing exist at least one reference space it is at rest with because of their relative stability of form. 
    Larger constellations of matter may comprise many physical features that are at rest with them.
    """@en .

  crmgeo:Q6i_rests_in_relation_to 
    a owl:ObjectProperty ;
    skos:prefLabel "Q6i rests in relation to"@en ;
    skos:notation "Q6i" ;
    rdfs:label "rests in relation to"@en ;
    rdfs:domain crm:E18_Physical_Thing;
    rdfs:range crmgeo:SP3_Reference_Space;
    owl:inverseOf crmgeo:Q6_is_at_rest_in_relation_to;
    rdfs:comment """This property associates an instance of Reference Space with the instance of Physical Thing that is at rest in it. For all instances of 
    Physical Thing exist at least one reference space it is at rest with because of their relative stability of form. Larger constellations 
    of matter may comprise many physical features that are at rest with them.
    """@en .

  crmgeo:Q7_describes 
    a owl:ObjectProperty ;
    skos:prefLabel "Q7 describes"@en ;
    skos:notation "Q7" ;
    rdfs:label "describes"@en ;
    rdfs:domain crmgeo:SP4_Spatial_Coordinate_Reference_System;
    rdfs:range crmgeo:SP3_Reference_Space;
    owl:inverseOf crmgeo:Q7i_is_described_by;
    rdfs:comment """This property associates an instance of Spatial Coordinate Reference System with the instance of Reference Space for which it can be used to describe locations."""@en .

  crmgeo:Q7i_is_described_by 
    a owl:ObjectProperty ;
    skos:prefLabel "Q7i is described by"@en ;
    skos:notation "Q7i" ;
    rdfs:label "is described by"@en ;
    rdfs:domain crmgeo:SP3_Reference_Space;
    rdfs:range crmgeo:SP4_Spatial_Coordinate_Reference_System;
    owl:inverseOf crmgeo:Q7_describes;
    rdfs:comment """This property associates an instance of Spatial Coordinate Reference System with the instance of Reference Space for which it can be used to describe locations."""@en .

  crmgeo:Q8_is_fixed_on 
    a owl:ObjectProperty ;
    skos:prefLabel "Q8 is fixed on"@en ;
    skos:notation "Q8" ;
    rdfs:label "is fixed on"@en ;
    rdfs:domain crmgeo:SP4_Spatial_Coordinate_Reference_System;
    rdfs:range crm:E26_Physical_Feature;
    owl:inverseOf crmgeo:Q8i_fixes;
    rdfs:comment """This property defines the physical reference features that ground a spatial coordinate reference system in the real world. 
    In surveying and geodesy this is part of the datum definition and is often a point identified by a physical feature on earth (sometimes monuments) 
    where the earth approximation ellipsoid touches the earth and one axis of the ellipsoid runs through.
    """@en .

  crmgeo:Q8i_fixes 
    a owl:ObjectProperty ;
    skos:prefLabel "Q8i fixes"@en ;
    skos:notation "Q8i" ;
    rdfs:label "fixes"@en ;
    rdfs:domain crm:E26_Physical_Feature;
    rdfs:range crmgeo:SP4_Spatial_Coordinate_Reference_System;
    owl:inverseOf crmgeo:Q8_is_fixed_on;
    rdfs:comment """This property defines the physical reference features that ground a spatial coordinate reference system in the real world. 
    In surveying and geodesy this is part of the datum definition and is often a point identified by a physical feature on earth (sometimes monuments) 
    where the earth approximation ellipsoid touches the earth and one axis of the ellipsoid runs through.
    """@en .

  crmgeo:Q9_is_expressed_in_terms_of 
    a owl:ObjectProperty ;
    skos:prefLabel "Q9 is expressed in terms of"@en ;
    skos:notation "Q9" ;
    rdfs:label "is expressed in terms of"@en ;
    rdfs:domain crmgeo:SP6_Declarative_Place;
    rdfs:range crmgeo:SP4_Spatial_Coordinate_Reference_System;
    owl:inverseOf crmgeo:Q9i_terms_express;
    rdfs:comment """This property defines the coordinate reference system in terms of which a Space Primitive is formulated."""@en .

  crmgeo:Q9i_terms_express 
    a owl:ObjectProperty ;
    skos:prefLabel "Q9i terms express"@en ;
    skos:notation "Q9i" ;
    rdfs:label "terms express"@en ;
    rdfs:domain crmgeo:SP4_Spatial_Coordinate_Reference_System;
    rdfs:range crmgeo:SP6_Declarative_Place;
    owl:inverseOf crmgeo:Q9_is_expressed_in_terms_of;
    rdfs:comment """This property defines the coordinate reference system in terms of which a Space Primitive is formulated."""@en .

  crmgeo:Q11_approximates_spacetime 
    a owl:ObjectProperty ;
    skos:prefLabel "Q11 approximates spacetime"@en ;
    skos:notation "Q11" ;
    rdfs:label "approximates spacetime"@en ;
    rdfs:domain crmgeo:SP7_Declarative_Spacetime_Volume;
    rdfs:range crmgeo:SP1_Phenomenal_Spacetime_Volume;
    owl:inverseOf crmgeo:Q11i_spacetime_is_approximated_by;
    rdfs:comment """This property approximates an Place which is defined in the same reference space. 
    The property does not state the quality or accuracy of the approximation, but states the intention to approximate the place.
    """@en .

  crmgeo:Q11i_spacetime_is_approximated_by 
    a owl:ObjectProperty ;
    skos:prefLabel "Q11i spacetime is approximated by"@en ;
    skos:notation "Q11i" ;
    rdfs:label "spacetime is approximated by"@en ;
    rdfs:domain crmgeo:SP1_Phenomenal_Spacetime_Volume;
    rdfs:range crmgeo:SP7_Declarative_Spacetime_Volume;
    owl:inverseOf crmgeo:Q11_approximates_spacetime;
    rdfs:comment """This property approximates an Place which is defined in the same reference space. 
    The property does not state the quality or accuracy of the approximation, but states the intention to approximate the place.
    """@en .

  crmgeo:Q13_approximates_time 
    a owl:ObjectProperty ;
    skos:prefLabel "Q13 approximates time"@en ;
    skos:notation "Q13" ;
    rdfs:label "approximates time"@en ;
    rdfs:domain crmgeo:SP10_DeclarativeTime-Span;
    rdfs:range crmgeo:SP13_Phenomenal_Time-Span;
    owl:inverseOf crmgeo:Q13i_time_is_approximated_by;
    rdfs:comment """This property approximates a Time-Span. The property does not state the quality or accuracy of the approximation, but states the intention to approximate the time span ."""@en .

  crmgeo:Q13i_time_is_approximated_by 
    a owl:ObjectProperty ;
    skos:prefLabel "Q13i time is approximated by"@en ;
    skos:notation "Q13i" ;
    rdfs:label "time is approximated by"@en ;
    rdfs:domain crmgeo:SP13_Phenomenal_Time-Span;
    rdfs:range crmgeo:SP10_DeclarativeTime-Span;
    owl:inverseOf crmgeo:Q13_approximates_time;
    rdfs:comment """This property approximates a Time-Span. The property does not state the quality or accuracy of the approximation, but states the intention to approximate the time span ."""@en .

  crmgeo:Q15_time_is_expressed_in_terms_of 
    a owl:ObjectProperty ;
    skos:prefLabel "Q15 time is expressed in terms of"@en ;
    skos:notation "Q15" ;
    rdfs:label "time is expressed in terms of"@en ;
    rdfs:domain crmgeo:SP10_DeclarativeTime-Span;
    rdfs:range crmgeo:SP11_Temporal_Reference_System;
    owl:inverseOf crmgeo:Q15i_time_is_expressed_in_terms_of;
    rdfs:comment """This property defines the temporal reference system in terms of which an Time Expression is formulated."""@en .

  crmgeo:Q15i_time_is_expressed_in_terms_of 
    a owl:ObjectProperty ;
    skos:prefLabel "Q15i time is expressed in terms of"@en ;
    skos:notation "Q15i" ;
    rdfs:label "time is expressed in terms of"@en ;
    rdfs:domain crmgeo:SP11_Temporal_Reference_System;
    rdfs:range crmgeo:SP10_DeclarativeTime-Span;
    owl:inverseOf crmgeo:Q15_time_is_expressed_in_terms_of;
    rdfs:comment """This property defines the temporal reference system in terms of which an Time Expression is formulated."""@en .

  crmgeo:Q17_time_is_expressed_in_terms_of 
    a owl:ObjectProperty ;
    skos:prefLabel "Q17 time is expressed in terms of"@en ;
    skos:notation "Q17" ;
    rdfs:label "time is expressed in terms of"@en ;
    rdfs:domain crmgeo:SP7_Declarative_Spacetime_Volume;
    rdfs:range crmgeo:SP11_Temporal_Reference_System;
    owl:inverseOf crmgeo:Q17i_time_is_expressed_in_terms_of;
    rdfs:comment """This property defines the temporal reference system in terms of which a Spacetime Volume Expression is formulated."""@en .

  crmgeo:Q17i_time_is_expressed_in_terms_of 
    a owl:ObjectProperty ;
    skos:prefLabel "Q17i time is expressed in terms of"@en ;
    skos:notation "Q17i" ;
    rdfs:label "time is expressed in terms of"@en ;
    rdfs:domain crmgeo:SP11_Temporal_Reference_System;
    rdfs:range crmgeo:SP7_Declarative_Spacetime_Volume;
    owl:inverseOf crmgeo:Q17_time_is_expressed_in_terms_of;
    rdfs:comment """This property defines the temporal reference system in terms of which a Spacetime Volume Expression is formulated."""@en .

  crmgeo:Q18_place_is_expressed_in_terms_of 
    a owl:ObjectProperty ;
    skos:prefLabel "Q18 place is expressed in terms of"@en ;
    skos:notation "Q18" ;
    rdfs:label "place is expressed in terms of"@en ;
    rdfs:domain crmgeo:SP7_Declarative_Spacetime_Volume;
    rdfs:range crmgeo:SP4_Spatial_Coordinate_Reference_System;
    owl:inverseOf crmgeo:Q18i_place_is_expressed_in_terms_of;
    rdfs:comment """This property defines the spatial coordinate reference system in terms of which a Spacetime Volume Expression is formulated."""@en .

  crmgeo:Q18i_place_is_expressed_in_terms_of 
    a owl:ObjectProperty ;
    skos:prefLabel "Q18i place is expressed in terms of"@en ;
    skos:notation "Q18i" ;
    rdfs:label "place is expressed in terms of"@en ;
    rdfs:domain crmgeo:SP4_Spatial_Coordinate_Reference_System;
    rdfs:range crmgeo:SP7_Declarative_Spacetime_Volume;
    owl:inverseOf crmgeo:Q18_place_is_expressed_in_terms_of;
    rdfs:comment """This property defines the spatial coordinate reference system in terms of which a Spacetime Volume Expression is formulated."""@en .

  crmgeo:Q19_has_reference_event 
    a owl:ObjectProperty ;
    skos:prefLabel "Q19 has reference event"@en ;
    skos:notation "Q19" ;
    rdfs:label "has reference event"@en ;
    rdfs:domain crmgeo:SP11_Temporal_Reference_System;
    rdfs:range crm:E5_Event;
    owl:inverseOf crmgeo:Q19i_has_reference_event;
    rdfs:comment """This property defines the reference event for a Temporal Reference System"""@en .

  crmgeo:Q19i_has_reference_event 
    a owl:ObjectProperty ;
    skos:prefLabel "Q19i has reference event"@en ;
    skos:notation "Q19i" ;
    rdfs:label "has reference event"@en ;
    rdfs:domain crm:E5_Event;
    rdfs:range crmgeo:SP11_Temporal_Reference_System;
    owl:inverseOf crmgeo:Q19_has_reference_event;
    rdfs:comment """This property defines the reference event for a Temporal Reference System"""@en .
}